WIP4

Definitions.v
@@ -11,21 +11,76 @@ Implicit Types X : var.
 (* *************************************************************** *)
 (** ** Description of types *)
 
+(* Finite and co-finite sets of constructors (nats) *)
+Inductive constructors : Type :=
+  | cons_finite : fset nat -> constructors
+  | cons_cofinite : fset nat -> constructors.
+
+Definition cons_universe :=
+  cons_cofinite \{}.
+
+Definition cons_disjoint cs1 cs2 :=
+  match cs1, cs2 with
+  | cons_finite f1, cons_finite f2 => disjoint f1 f2
+  | cons_finite f1, cons_cofinite f2 => subset f1 f2
+  | cons_cofinite f1, cons_finite f2 => subset f2 f1
+  | cons_cofinite f1, cons_cofinite f2 => False
+  end.
+
+Definition cons_union cs1 cs2 := 
+  match cs1, cs2 with
+  | cons_finite f1, cons_finite f2 => cons_finite (f1 \u f2)
+  | cons_finite f1, cons_cofinite f2 => cons_cofinite (f2 \- f1)
+  | cons_cofinite f1, cons_finite f2 => cons_cofinite (f1 \- f2)
+  | cons_cofinite f1, cons_cofinite f2 => cons_cofinite (f1 \n f2)
+  end.
+
+Definition cons_inter cs1 cs2 := 
+  match cs1, cs2 with
+  | cons_finite f1, cons_finite f2 => cons_finite (f1 \n f2)
+  | cons_finite f1, cons_cofinite f2 => cons_finite (f1 \- f2)
+  | cons_cofinite f1, cons_finite f2 => cons_finite (f2 \- f1)
+  | cons_cofinite f1, cons_cofinite f2 => cons_cofinite (f1 \u f2)
+  end.
+
+Definition cons_subset cs1 cs2 :=
+  match cs1, cs2 with
+  | cons_finite f1, cons_finite f2 => subset f1 f2
+  | cons_finite f1, cons_cofinite f2 => disjoint f1 f2
+  | cons_cofinite f1, cons_finite f2 => False
+  | cons_cofinite f1, cons_cofinite f2 => subset f2 f1
+  end.
+
+Definition cons_diff cs1 cs2 := 
+  match cs1, cs2 with
+  | cons_finite f1, cons_finite f2 => cons_finite (f1 \- f2)
+  | cons_finite f1, cons_cofinite f2 => cons_finite (f1 \n f2)
+  | cons_cofinite f1, cons_finite f2 => cons_cofinite (f1 \u f2)
+  | cons_cofinite f1, cons_cofinite f2 => cons_finite (f2 \- f1)
+  end.
+
+Definition cons_non_empty cs :=
+  match cs with
+  | cons_finite f => exists c, c \in f
+  | cons_cofinite _ => True
+  end.
+
 (* Kinds *)
-Inductive kind : Set :=
-  | kind_type : kind
-  | kind_row : kind.
+Inductive knd : Type :=
+  | knd_type : knd
+  | knd_row : constructors -> knd.
 
 (** Representation of pre-types *)
 
-Inductive typ : Set :=
+Inductive typ : Type :=
   | typ_bvar : nat -> typ
   | typ_fvar : var -> typ
   | typ_constructor : nat -> typ -> typ
+  | typ_or : typ -> typ -> typ
   | typ_variant : typ -> typ -> typ
   | typ_arrow : typ -> typ -> typ
-  | typ_top : typ
-  | typ_bot : typ
+  | typ_top : constructors -> typ
+  | typ_bot : constructors -> typ
   | typ_meet : typ -> typ -> typ
   | typ_join : typ -> typ -> typ.
 
@@ -33,10 +88,17 @@ Inductive typ : Set :=
 
 Definition typ_def := typ_bvar 0.
 
+Definition typ_nil := typ_bot (cons_finite \{}).
+
+Definition typ_row cs T R :=
+  fold_right
+    (fun c acc => typ_or (typ_constructor c T) acc)
+    R cs.
+
 (** Type schemes. *)
 
-Record sch : Set := Sch { 
-  sch_kinds : list kind ;
+Record sch : Type := Sch { 
+  sch_kinds : list knd ;
   sch_type  : typ }.
 
 Definition sch_arity M := length (sch_kinds M).
@@ -48,10 +110,11 @@ Fixpoint typ_open (T : typ) (Vs : list typ) {struct T} : typ :=
   | typ_bvar i => nth i Vs typ_def
   | typ_fvar x => typ_fvar x 
   | typ_constructor c T => typ_constructor c (typ_open T Vs)
+  | typ_or T1 T2 => typ_or (typ_open T1 Vs) (typ_open T2 Vs)
   | typ_variant T1 T2 => typ_variant (typ_open T1 Vs) (typ_open T2 Vs)
   | typ_arrow T1 T2 => typ_arrow (typ_open T1 Vs) (typ_open T2 Vs)
-  | typ_top => typ_top
-  | typ_bot => typ_bot
+  | typ_top cs => typ_top cs
+  | typ_bot cs => typ_bot cs
   | typ_meet T1 T2 => typ_meet (typ_open T1 Vs) (typ_open T2 Vs)
   | typ_join T1 T2 => typ_join (typ_open T1 Vs) (typ_open T2 Vs)
   end.
@@ -80,6 +143,15 @@ Notation "M ^ Xs" :=
 Bind Scope typ_scope with typ.
 Open Scope typ_scope.
 
+(** Well-formed kinds *)
+Inductive kind : knd -> Prop :=
+  | kind_type : kind knd_type
+  | kind_row : forall cs,
+      cons_non_empty cs -> kind (knd_row cs).
+
+Definition kinds n (L : list knd) :=
+  n = length L /\ Forall kind L.
+
 (** Locally closed types *)
 
 Inductive type : typ -> Prop :=
@@ -88,6 +160,10 @@ Inductive type : typ -> Prop :=
   | type_constructor : forall c T,
       type T ->
       type (typ_constructor c T)
+  | type_or : forall T1 T2,
+      type T1 ->
+      type T2 ->
+      type (typ_or T1 T2)
   | type_variant : forall T1 T2,
       type T1 ->
       type T2 ->
@@ -96,8 +172,10 @@ Inductive type : typ -> Prop :=
       type T1 -> 
       type T2 -> 
       type (typ_arrow T1 T2)
-  | type_top : type (typ_top)
-  | type_bot : type (typ_bot)
+  | type_top : forall cs,
+      type (typ_top cs)
+  | type_bot : forall cs,
+      type (typ_bot cs)
   | type_meet : forall T1 T2,
       type T1 ->
       type T2 ->
@@ -122,21 +200,23 @@ Definition type_body n T :=
 (** Definition of a well-formed scheme *)
 
 Definition scheme M :=
-  type_body (sch_arity M) (sch_type M).
+  type_body (sch_arity M) (sch_type M)
+  /\ kinds (sch_arity M) (sch_kinds M).
 
 (* ************************************************************** *)
 (** ** Description of terms *)
 
 (** Representation of pre-terms *)
 
-Inductive trm : Set :=
+Inductive trm : Type :=
   | trm_bvar : nat -> trm
   | trm_fvar : var -> trm
   | trm_abs : trm -> trm
   | trm_let : trm -> trm -> trm
   | trm_app : trm -> trm -> trm
   | trm_constructor : nat -> trm -> trm
-  | trm_match : trm -> nat -> trm -> trm -> trm
+  | trm_match : trm -> list nat -> trm -> trm -> trm
+  | trm_destruct : trm -> list nat -> trm -> trm
   | trm_absurd : trm -> trm.
 
 Fixpoint trm_open_rec (k : nat) (u : trm) (t : trm) {struct t} : trm :=
@@ -150,10 +230,13 @@ Fixpoint trm_open_rec (k : nat) (u : trm) (t : trm) {struct t} : trm :=
       trm_app (trm_open_rec k u t1) (trm_open_rec k u t2)
   | trm_constructor c t =>
       trm_constructor c (trm_open_rec k u t)
-  | trm_match t1 c t2 t3 =>
-      trm_match (trm_open_rec k u t1) c
+  | trm_match t1 cs t2 t3 =>
+      trm_match (trm_open_rec k u t1) cs
                 (trm_open_rec (S k) u t2)
                 (trm_open_rec (S k) u t3)
+  | trm_destruct t1 cs t2 =>
+      trm_destruct (trm_open_rec k u t1) cs
+                   (trm_open_rec (S k) u t2)
   | trm_absurd t1 => trm_absurd (trm_open_rec k u t1)
   end.
 
@@ -182,11 +265,15 @@ Inductive term : trm -> Prop :=
   | term_constructor : forall c t,
       term t ->
       term (trm_constructor c t)
-  | term_match : forall L t1 c t2 t3,
+  | term_match : forall L t1 cs t2 t3,
       term t1 ->
       (forall x, x \notin L -> term (t2 ^ x)) ->
       (forall x, x \notin L -> term (t3 ^ x)) ->
-      term (trm_match t1 c t2 t3)
+      term (trm_match t1 cs t2 t3)
+  | term_destruct : forall L t1 cs t2,
+      term t1 ->
+      (forall x, x \notin L -> term (t2 ^ x)) ->
+      term (trm_destruct t1 cs t2)
   | term_absurd : forall t,
       term t ->
       term (trm_absurd t).
@@ -204,18 +291,18 @@ Definition term_body t :=
  [X ~:: T] is a kinding asumption and [x ~: T] is
  a typing assumption *)
 
-Inductive bind : Set :=
-  | bind_kind : kind -> bind
+Inductive bind : Type :=
+  | bind_knd : knd -> bind
   | bind_typ : sch -> bind.
 
-Definition bind_kinds Xs Ks :=
-  map bind_kind (Xs ~* Ks).
+Definition bind_knds Xs Ks :=
+  map bind_knd (Xs ~* Ks).
 
-Notation "X ~:: K" := (X ~ bind_kind K)
+Notation "X ~:: K" := (X ~ bind_knd K)
   (at level 23, left associativity) : env_scope.
 Notation "x ~: T" := (x ~ bind_typ T)
   (at level 23, left associativity) : env_scope.
-Notation "Xs ~::* Ks" := (map bind_kind (Xs ~* Ks))
+Notation "Xs ~::* Ks" := (map bind_knd (Xs ~* Ks))
   (at level 23, left associativity) : env_scope.
 
 (** Pre-environment is an associative list of bindings. *)
@@ -227,8 +314,9 @@ Definition env := LibEnv.env bind.
 Inductive environment : env -> Prop :=
   | environment_empty :
       environment empty
-  | environment_kind : forall E X K,
+  | environment_knd : forall E X K,
       environment E ->
+      kind K ->
       X # E ->
       environment (E & X ~:: K)
   | environment_typ : forall E x M,
@@ -242,38 +330,46 @@ Inductive environment : env -> Prop :=
 
 (** The kinding relation *)
 
-Inductive kinding : env -> typ -> kind -> Prop :=
+Inductive kinding : env -> typ -> knd -> Prop :=
   | kinding_var : forall K E X,
       environment E ->
-      binds X (bind_kind K) E ->
+      binds X (bind_knd K) E ->
       kinding E (typ_fvar X) K
   | kinding_constructor : forall E c T,
-      kinding E T kind_type ->
-      kinding E (typ_constructor c T) kind_row
+      kinding E T knd_type ->
+      kinding E (typ_constructor c T)
+              (knd_row (cons_finite \{c}))
+  | kinding_or : forall E cs1 T1 cs2 T2,
+      cons_disjoint cs1 cs2 ->
+      kinding E T1 (knd_row cs1) ->
+      kinding E T2 (knd_row cs2) ->
+      kinding E (typ_or T1 T2) (knd_row (cons_union cs1 cs2))
   | kinding_variant : forall E T1 T2,
-      kinding E T1 kind_row ->
-      kinding E T2 kind_row ->
-      kinding E (typ_variant T1 T2) kind_type
+      kinding E T1 (knd_row cons_universe) ->
+      kinding E T2 (knd_row cons_universe) ->
+      kinding E (typ_variant T1 T2) knd_type
   | kinding_arrow : forall E T1 T2,
-      kinding E T1 kind_type -> 
-      kinding E T2 kind_type -> 
-      kinding E (typ_arrow T1 T2) kind_type
-  | kinding_top : forall E,
+      kinding E T1 knd_type -> 
+      kinding E T2 knd_type -> 
+      kinding E (typ_arrow T1 T2) knd_type
+  | kinding_top : forall E cs,
+      cons_non_empty cs ->
       environment E ->
-      kinding E typ_top kind_row
-  | kinding_bot : forall E,
+      kinding E (typ_top cs) (knd_row cs)
+  | kinding_bot : forall E cs,
+      cons_non_empty cs ->
       environment E ->
-      kinding E typ_bot kind_row
-  | kinding_meet : forall E T1 T2,
-      kinding E T1 kind_row ->
-      kinding E T2 kind_row ->
-      kinding E (typ_meet T1 T2) kind_row
-  | kinding_join : forall E T1 T2,
-      kinding E T1 kind_row ->
-      kinding E T2 kind_row ->
-      kinding E (typ_join T1 T2) kind_row.
+      kinding E (typ_bot cs) (knd_row cs)
+  | kinding_meet : forall E cs T1 T2,
+      kinding E T1 (knd_row cs) ->
+      kinding E T2 (knd_row cs) ->
+      kinding E (typ_meet T1 T2) (knd_row cs)
+  | kinding_join : forall E cs T1 T2,
+      kinding E T1 (knd_row cs) ->
+      kinding E T2 (knd_row cs) ->
+      kinding E (typ_join T1 T2) (knd_row cs).
 
-Inductive kindings : env -> nat -> list typ -> list kind -> Prop :=
+Inductive kindings : env -> nat -> list typ -> list knd -> Prop :=
   | kindings_nil : forall E,
       environment E ->
       kindings E 0 nil nil
@@ -285,7 +381,8 @@ Inductive kindings : env -> nat -> list typ -> list kind -> Prop :=
 Definition kinding_body E n Ks T :=
   exists L, forall Xs, 
   fresh L n Xs ->
-  kinding (E & Xs ~::* Ks) (typ_open_vars T Xs) kind_type.
+  kinds n Ks /\
+  kinding (E & Xs ~::* Ks) (typ_open_vars T Xs) knd_type.
 
 Definition kinding_scheme E M :=
   kinding_body E (sch_arity M) (sch_kinds M) (sch_type M).
@@ -299,6 +396,7 @@ Inductive kinding_env : env -> Prop :=
       kinding_env empty
   | kinding_env_kind : forall E X K,
       kinding_env E ->
+      kind K ->
       X # E ->
       kinding_env (E & X ~:: K)
   | kinding_env_typ : forall E x M,
@@ -312,128 +410,235 @@ Inductive kinding_env : env -> Prop :=
 
 (** Equality relation on types *)
 
-Inductive type_equal : env -> typ -> typ -> kind -> Prop :=
+Inductive type_equal : env -> typ -> typ -> knd -> Prop :=
   | type_equal_var : forall E x K,
       environment E ->
-      binds x (bind_kind K) E ->
+      binds x (bind_knd K) E ->
       type_equal E (typ_fvar x) (typ_fvar x) K
   | type_equal_constructor : forall E c T T',
-      type_equal E T T' kind_type ->
-      type_equal E (typ_constructor c T) (typ_constructor c T') kind_row
+      type_equal E T T' knd_type ->
+      type_equal E (typ_constructor c T) (typ_constructor c T')
+                 (knd_row (cons_finite \{c}))
+  | type_equal_or : forall E cs1 T1 T1' cs2 T2 T2',
+      cons_disjoint cs1 cs2 ->
+      type_equal E T1 T1' (knd_row cs1) ->
+      type_equal E T2 T2' (knd_row cs2) ->
+      type_equal E (typ_or T1 T2) (typ_or T1' T2')
+                 (knd_row (cons_union cs1 cs2))
   | type_equal_variant : forall E T1 T1' T2 T2',
-      type_equal E T1 T1' kind_row ->
-      type_equal E T2 T2' kind_row ->
-      type_equal E (typ_variant T1 T2) (typ_variant T1' T2') kind_type
+      type_equal E T1 T1' (knd_row cons_universe) ->
+      type_equal E T2 T2' (knd_row cons_universe) ->
+      type_equal E (typ_variant T1 T2) (typ_variant T1' T2') knd_type
   | type_equal_arrow : forall E T1 T1' T2 T2',
-      type_equal E T1 T1' kind_type ->
-      type_equal E T2 T2' kind_type ->
-      type_equal E (typ_arrow T1 T2) (typ_arrow T1' T2') kind_type
-  | type_equal_top : forall E,
+      type_equal E T1 T1' knd_type ->
+      type_equal E T2 T2' knd_type ->
+      type_equal E (typ_arrow T1 T2) (typ_arrow T1' T2') knd_type
+  | type_equal_top : forall E cs,
       environment E ->
-      type_equal E typ_top typ_top kind_row
-  | type_equal_bot : forall E,
+      cons_non_empty cs ->
+      type_equal E (typ_top cs) (typ_top cs) (knd_row cs)
+  | type_equal_bot : forall E cs,
       environment E ->
-      type_equal E typ_bot typ_bot kind_row
-  | type_equal_meet : forall E T1 T1' T2 T2',
-      type_equal E T1 T1' kind_row ->
-      type_equal E T2 T2' kind_row -> 
-      type_equal E (typ_meet T1 T2) (typ_meet T1' T2') kind_row
-  | type_equal_join : forall E T1 T1' T2 T2',
-      type_equal E T1 T1' kind_row ->
-      type_equal E T2 T2' kind_row ->
-      type_equal E (typ_join T1 T2) (typ_join T1' T2') kind_row
+      cons_non_empty cs ->
+      type_equal E (typ_bot cs) (typ_bot cs) (knd_row cs)
+  | type_equal_meet : forall E cs T1 T1' T2 T2',
+      type_equal E T1 T1' (knd_row cs) ->
+      type_equal E T2 T2' (knd_row cs) -> 
+      type_equal E (typ_meet T1 T2) (typ_meet T1' T2') (knd_row cs)
+  | type_equal_join : forall E cs T1 T1' T2 T2',
+      type_equal E T1 T1' (knd_row cs) ->
+      type_equal E T2 T2' (knd_row cs) ->
+      type_equal E (typ_join T1 T2) (typ_join T1' T2') (knd_row cs)
   | type_equal_trans : forall E T1 T2 T3 K,
       type_equal E T1 T2 K ->
       type_equal E T2 T3 K ->
       type_equal E T1 T3 K
-  | type_equal_meet_commutative : forall E T1 T2,
-      kinding E T1 kind_row ->
-      kinding E T2 kind_row ->
-      type_equal E (typ_meet T1 T2) (typ_meet T2 T1) kind_row
-  | type_equal_meet_associative_l : forall E T1 T2 T3,
-      kinding E T1 kind_row ->
-      kinding E T2 kind_row ->
-      kinding E T3 kind_row ->
+  | type_equal_or_commutative : forall E cs1 T1 cs2 T2,
+      cons_disjoint cs1 cs2 ->
+      kinding E T1 (knd_row cs1) ->
+      kinding E T2 (knd_row cs2) ->
+      type_equal E (typ_or T1 T2) (typ_or T2 T1)
+                 (knd_row (cons_union cs1 cs2))
+  | type_equal_or_associative_l : forall E cs1 T1 cs2 T2 cs3 T3,
+      cons_disjoint cs1 cs2 ->
+      cons_disjoint cs2 cs3 ->
+      cons_disjoint cs1 cs3 ->
+      kinding E T1 (knd_row cs1) ->
+      kinding E T2 (knd_row cs2) ->
+      kinding E T3 (knd_row cs3) ->
+      type_equal E (typ_or T1 (typ_or T2 T3))
+                 (typ_or (typ_or T1 T2) T3)
+                 (knd_row (cons_union cs1 (cons_union cs2 cs3)))
+  | type_equal_or_associative_r : forall E cs1 T1 cs2 T2 cs3 T3,
+      cons_disjoint cs1 cs2 ->
+      cons_disjoint cs2 cs3 ->
+      cons_disjoint cs1 cs3 ->
+      kinding E T1 (knd_row cs1) ->
+      kinding E T2 (knd_row cs2) ->
+      kinding E T3 (knd_row cs3) ->
+      type_equal E (typ_or (typ_or T1 T2) T3)
+                 (typ_or T1 (typ_or T2 T3))
+                 (knd_row (cons_union cs1 (cons_union cs2 cs3)))
+  | type_equal_or_bot_l : forall E cs1 cs2,
+      environment E ->
+      cons_disjoint cs1 cs2 ->
+      cons_non_empty cs1 ->
+      cons_non_empty cs2 ->
+      type_equal E (typ_or (typ_bot cs1) (typ_bot cs2))
+                 (typ_bot (cons_union cs1 cs2))
+                 (knd_row (cons_union cs1 cs2))
+  | type_equal_or_bot_r : forall E cs1 cs2,
+      environment E ->
+      cons_disjoint cs1 cs2 ->
+      cons_non_empty cs1 ->
+      cons_non_empty cs2 ->
+      type_equal E (typ_bot (cons_union cs1 cs2))
+                 (typ_or (typ_bot cs1) (typ_bot cs2))
+                 (knd_row (cons_union cs1 cs2))
+  | type_equal_or_top_l : forall E cs1 cs2,
+      environment E ->
+      cons_disjoint cs1 cs2 ->
+      cons_non_empty cs1 ->
+      cons_non_empty cs2 ->
+      type_equal E (typ_or (typ_top cs1) (typ_top cs2))
+                 (typ_top (cons_union cs1 cs2))
+                 (knd_row (cons_union cs1 cs2))
+  | type_equal_or_top_r : forall E cs1 cs2,
+      environment E ->
+      cons_disjoint cs1 cs2 ->
+      cons_non_empty cs1 ->
+      cons_non_empty cs2 ->
+      type_equal E (typ_top (cons_union cs1 cs2))
+                 (typ_or (typ_top cs1) (typ_top cs2))
+                 (knd_row (cons_union cs1 cs2))
+  | type_equal_or_meet_distribution_l : forall E cs1 T1 cs2 T2 T3 T4,
+      cons_disjoint cs1 cs2 ->
+      kinding E T1 (knd_row cs1) ->
+      kinding E T2 (knd_row cs2) ->
+      kinding E T3 (knd_row cs1) ->
+      kinding E T4 (knd_row cs2) ->
+      type_equal E (typ_or (typ_meet T1 T3) (typ_meet T2 T4))
+                 (typ_meet (typ_or T1 T2) (typ_or T3 T4))
+                 (knd_row (cons_union cs1 cs2))
+  | type_equal_or_meet_distribution_r : forall E cs1 T1 cs2 T2 T3 T4,
+      cons_disjoint cs1 cs2 ->
+      kinding E T1 (knd_row cs1) ->
+      kinding E T2 (knd_row cs2) ->
+      kinding E T3 (knd_row cs1) ->
+      kinding E T4 (knd_row cs2) ->
+      type_equal E (typ_meet (typ_or T1 T2) (typ_or T3 T4))
+                 (typ_or (typ_meet T1 T3) (typ_meet T2 T4))
+                 (knd_row (cons_union cs1 cs2))
+  | type_equal_or_join_distribution_l : forall E cs1 T1 cs2 T2 T3 T4,
+      cons_disjoint cs1 cs2 ->
+      kinding E T1 (knd_row cs1) ->
+      kinding E T2 (knd_row cs2) ->
+      kinding E T3 (knd_row cs1) ->
+      kinding E T4 (knd_row cs2) ->
+      type_equal E (typ_or (typ_join T1 T3) (typ_join T2 T4))
+                 (typ_join (typ_or T1 T2) (typ_or T3 T4))
+                 (knd_row (cons_union cs1 cs2))
+  | type_equal_or_join_distribution_r : forall E cs1 T1 cs2 T2 T3 T4,
+      cons_disjoint cs1 cs2 ->
+      kinding E T1 (knd_row cs1) ->
+      kinding E T2 (knd_row cs2) ->
+      kinding E T3 (knd_row cs1) ->
+      kinding E T4 (knd_row cs2) ->
+      type_equal E (typ_join (typ_or T1 T2) (typ_or T3 T4))
+                 (typ_or (typ_join T1 T3) (typ_join T2 T4))
+                 (knd_row (cons_union cs1 cs2))
+  | type_equal_meet_commutative : forall E cs T1 T2,
+      kinding E T1 (knd_row cs) ->
+      kinding E T2 (knd_row cs) ->
+      type_equal E (typ_meet T1 T2) (typ_meet T2 T1) (knd_row cs)
+  | type_equal_meet_associative_l : forall E cs T1 T2 T3,
+      kinding E T1 (knd_row cs) ->
+      kinding E T2 (knd_row cs) ->
+      kinding E T3 (knd_row cs) ->
       type_equal E (typ_meet T1 (typ_meet T2 T3))
-                 (typ_meet (typ_meet T1 T2) T3) kind_row
-  | type_equal_meet_associative_r : forall E T1 T2 T3,
-      kinding E T1 kind_row ->
-      kinding E T2 kind_row ->
-      kinding E T3 kind_row ->
+                 (typ_meet (typ_meet T1 T2) T3) (knd_row cs)
+  | type_equal_meet_associative_r : forall E cs T1 T2 T3,
+      kinding E T1 (knd_row cs) ->
+      kinding E T2 (knd_row cs) ->
+      kinding E T3 (knd_row cs) ->
       type_equal E (typ_meet (typ_meet T1 T2) T3)
-                 (typ_meet T1 (typ_meet T2 T3)) kind_row
-  | type_equal_meet_identity_l : forall E T,
-      kinding E T kind_row ->
-      type_equal E (typ_meet T typ_top) T kind_row
-  | type_equal_meet_identity_r : forall E T,
-      kinding E T kind_row ->
-      type_equal E T (typ_meet T typ_top) kind_row
-  | type_equal_meet_absorption_l : forall E T1 T2,
-      kinding E T1 kind_row ->
-      kinding E T2 kind_row ->
-      type_equal E (typ_meet T1 (typ_join T1 T2)) T1 kind_row
-  | type_equal_meet_absorption_r : forall E T1 T2,
-      kinding E T1 kind_row ->
-      kinding E T2 kind_row ->
-      type_equal E T1 (typ_meet T1 (typ_join T1 T2)) kind_row
-  | type_equal_meet_distribution_l : forall E T1 T2 T3,
-      kinding E T1 kind_row ->
-      kinding E T2 kind_row ->
-      kinding E T3 kind_row ->
+                 (typ_meet T1 (typ_meet T2 T3)) (knd_row cs)
+  | type_equal_meet_identity_l : forall E cs T,
+      kinding E T (knd_row cs) ->
+      type_equal E (typ_meet T (typ_top cs)) T (knd_row cs)
+  | type_equal_meet_identity_r : forall E cs T,
+      kinding E T (knd_row cs) ->
+      type_equal E T (typ_meet T (typ_top cs)) (knd_row cs)
+  | type_equal_meet_absorption_l : forall E cs T1 T2,
+      kinding E T1 (knd_row cs) ->
+      kinding E T2 (knd_row cs) ->
+      type_equal E (typ_meet T1 (typ_join T1 T2)) T1 (knd_row cs)
+  | type_equal_meet_absorption_r : forall E cs T1 T2,
+      kinding E T1 (knd_row cs) ->
+      kinding E T2 (knd_row cs) ->
+      type_equal E T1 (typ_meet T1 (typ_join T1 T2)) (knd_row cs)
+  | type_equal_meet_distribution_l : forall E cs T1 T2 T3,
+      kinding E T1 (knd_row cs) ->
+      kinding E T2 (knd_row cs) ->
+      kinding E T3 (knd_row cs) ->
       type_equal E (typ_meet (typ_join T1 T2) (typ_join T1 T3))
-                 (typ_join T1 (typ_meet T2 T3)) kind_row
-  | type_equal_meet_distribution_r : forall E T1 T2 T3,
-      kinding E T1 kind_row ->
-      kinding E T2 kind_row ->
-      kinding E T3 kind_row ->
+                 (typ_join T1 (typ_meet T2 T3)) (knd_row cs)
+  | type_equal_meet_distribution_r : forall E cs T1 T2 T3,
+      kinding E T1 (knd_row cs) ->
+      kinding E T2 (knd_row cs) ->
+      kinding E T3 (knd_row cs) ->
       type_equal E (typ_join T1 (typ_meet T2 T3))
-                 (typ_meet (typ_join T1 T2) (typ_join T1 T3)) kind_row
-  | type_equal_join_commutative : forall E T1 T2,
-      kinding E T1 kind_row ->
-      kinding E T2 kind_row ->
-      type_equal E (typ_join T1 T2) (typ_join T2 T1) kind_row
-  | type_equal_join_associative_l : forall E T1 T2 T3,
-      kinding E T1 kind_row ->
-      kinding E T2 kind_row ->
-      kinding E T3 kind_row ->
+                 (typ_meet (typ_join T1 T2) (typ_join T1 T3))
+                 (knd_row cs)
+  | type_equal_join_commutative : forall E cs T1 T2,
+      kinding E T1 (knd_row cs) ->
+      kinding E T2 (knd_row cs) ->
+      type_equal E (typ_join T1 T2) (typ_join T2 T1) (knd_row cs)
+  | type_equal_join_associative_l : forall E cs T1 T2 T3,
+      kinding E T1 (knd_row cs) ->
+      kinding E T2 (knd_row cs) ->
+      kinding E T3 (knd_row cs) ->
       type_equal E (typ_join T1 (typ_join T2 T3))
-                 (typ_join (typ_join T1 T2) T3) kind_row
-  | type_equal_join_associative_r : forall E T1 T2 T3,
-      kinding E T1 kind_row ->
-      kinding E T2 kind_row ->
-      kinding E T3 kind_row ->
+                 (typ_join (typ_join T1 T2) T3) (knd_row cs)
+  | type_equal_join_associative_r : forall E cs T1 T2 T3,
+      kinding E T1 (knd_row cs) ->
+      kinding E T2 (knd_row cs) ->
+      kinding E T3 (knd_row cs) ->
       type_equal E (typ_join (typ_join T1 T2) T3)
-                 (typ_join T1 (typ_join T2 T3)) kind_row
-  | type_equal_join_identity_l : forall E T,
-      kinding E T kind_row ->
-      type_equal E (typ_join T typ_bot) T kind_row
-  | type_equal_join_identity_r : forall E T,
-      kinding E T kind_row ->
-      type_equal E T (typ_join T typ_bot) kind_row
-  | type_equal_join_absorption_l : forall E T1 T2,
-      kinding E T1 kind_row ->
-      kinding E T2 kind_row ->
-      type_equal E (typ_join T1 (typ_meet T1 T2)) T1 kind_row
-  | type_equal_join_absorption_r : forall E T1 T2,
-      kinding E T1 kind_row ->
-      kinding E T2 kind_row ->
-      type_equal E T1 (typ_join T1 (typ_meet T1 T2)) kind_row
-  | type_equal_join_distribution_l : forall E T1 T2 T3,
-      kinding E T1 kind_row ->
-      kinding E T2 kind_row ->
-      kinding E T3 kind_row ->
+                 (typ_join T1 (typ_join T2 T3)) (knd_row cs)
+  | type_equal_join_identity_l : forall E cs T,
+      kinding E T (knd_row cs) ->
+      type_equal E (typ_join T (typ_bot cs)) T (knd_row cs)
+  | type_equal_join_identity_r : forall E cs T,
+      kinding E T (knd_row cs) ->
+      type_equal E T (typ_join T (typ_bot cs)) (knd_row cs)
+  | type_equal_join_absorption_l : forall E cs T1 T2,
+      kinding E T1 (knd_row cs) ->
+      kinding E T2 (knd_row cs) ->
+      type_equal E (typ_join T1 (typ_meet T1 T2)) T1 (knd_row cs)
+  | type_equal_join_absorption_r : forall E cs T1 T2,
+      kinding E T1 (knd_row cs) ->
+      kinding E T2 (knd_row cs) ->
+      type_equal E T1 (typ_join T1 (typ_meet T1 T2)) (knd_row cs)
+  | type_equal_join_distribution_l : forall E cs T1 T2 T3,
+      kinding E T1 (knd_row cs) ->
+      kinding E T2 (knd_row cs) ->
+      kinding E T3 (knd_row cs) ->
       type_equal E (typ_join T1 (typ_meet T2 T3))
-                 (typ_meet (typ_join T1 T2) (typ_join T1 T3)) kind_row
-  | type_equal_join_distribution : forall E T1 T2 T3,
-      kinding E T1 kind_row -> 
-      kinding E T2 kind_row ->
-      kinding E T3 kind_row ->
+                 (typ_meet (typ_join T1 T2) (typ_join T1 T3))
+                 (knd_row cs)
+  | type_equal_join_distribution : forall E cs T1 T2 T3,
+      kinding E T1 (knd_row cs) -> 
+      kinding E T2 (knd_row cs) ->
+      kinding E T3 (knd_row cs) ->
       type_equal E (typ_meet (typ_join T1 T2) (typ_join T1 T3))
-                 (typ_join T1 (typ_meet T2 T3)) kind_row.
+                 (typ_join T1 (typ_meet T2 T3)) (knd_row cs).
 
 
 Definition subtype E T1 T2 :=
-  type_equal E T1 (typ_join T1 T2) kind_row.
+  type_equal E T1 (typ_meet T1 T2) (knd_row cons_universe).
+
+Notation "E ||= T1 -<: T2" := (subtype E T1 T2) (at level 60).
 
 Inductive typing : env -> trm -> typ -> Prop :=
   | typing_var : forall E x M Us, 
@@ -442,9 +647,9 @@ Inductive typing : env -> trm -> typ -> Prop :=
       kindings E (sch_arity M) Us (sch_kinds M) ->
       typing E (trm_fvar x) (M ^^ Us)
   | typing_abs : forall L E T1 T2 t1, 
-      kinding E T1 kind_type ->
       (forall x, x \notin L -> 
         typing (E & x ~ bind_typ (Sch nil T1)) (t1 ^ x) T2) -> 
+      kinding E T1 knd_type ->
       typing E (trm_abs t1) (typ_arrow T1 T2)
   | typing_app : forall E S T t1 t2, 
       typing E t1 (typ_arrow S T) ->
@@ -459,30 +664,55 @@ Inductive typing : env -> trm -> typ -> Prop :=
       typing E (trm_let t1 t2) T2
   | typing_constructor : forall c E T1 T2 T3 t,
       typing E t T1 ->
-      subtype E (typ_constructor c T1) T2 ->
-      subtype E T2 T3 ->
+      E ||= (typ_or (typ_constructor c T1)
+                   (typ_bot (cons_cofinite \{c})))
+           -<: T2 ->
+      (E ||= T2 -<: T3) ->
       typing E (trm_constructor c t) (typ_variant T3 T2)
-  | typing_match : forall c L E T1 T2 T3 T4 T5 T6 t1 t2 t3,
+  | typing_match : forall cs L E T1 T2 T3 T4 T5
+                          T6 T7 T8 T9 T10 t1 t2 t3,
       typing E t1 (typ_variant T1 T2) ->
-      (forall x, x \notin L -> 
-         typing (E & x ~ bind_typ (Sch nil T3)) (t2 ^ x) T4) ->
+      (forall x, x \notin L ->
+         typing (E & x ~: (Sch nil (typ_variant T3 T4)))
+                (t2 ^ x) T5) ->
       (forall y, y \notin L -> 
-         typing (E & y ~ bind_typ (Sch nil (typ_variant T5 T6)))
-                (t3 ^ y) T4) ->
-      subtype E T1 (typ_join (typ_constructor c T3) T6) ->
-      subtype E T2 T1 ->
-      subtype E T6 T5 ->
-      typing E (trm_match t1 c t2 t3) T4
-  | typing_absurd : forall E T1 T2 T3 t1,
-      kinding E T3 kind_type ->
+         typing (E & y ~: (Sch nil (typ_variant T6 T7)))
+                (t3 ^ y) T5) ->
+      kinding E T10 knd_type ->
+      E ||= T1 -<: (typ_or T8 T9) ->
+      E ||= (typ_or T8
+                   (typ_bot (cons_cofinite (from_list cs))))
+           -<: (typ_row cs T10
+                       (typ_bot (cons_cofinite (from_list cs)))) ->
+      E ||= (typ_or T8 (typ_bot (cons_cofinite (from_list cs))))
+           -<: T4 ->
+      E ||= (typ_or (typ_bot (cons_finite (from_list cs))) T9)
+           -<: T7 ->
+      E ||= T2 -<: T1 ->
+      E ||= T4 -<: T3 ->
+      E ||= T7 -<: T6 ->
+      typing E (trm_match t1 cs t2 t3) T5
+  | typing_destruct : forall cs L E T1 T2 T3 T4 t1 t2,
       typing E t1 (typ_variant T1 T2) ->
-      subtype E typ_bot T2 ->
-      subtype E T2 T1 ->
+      (forall x, x \notin L ->
+         typing (E & x ~: (Sch nil T3))
+                (t2 ^ x) T4) ->
+      kinding E T3 knd_type ->
+      E ||= T1 -<: (typ_row cs T3
+                    (typ_bot (cons_cofinite (from_list cs)))) ->
+      E ||= T2 -<: T1 ->
+      typing E (trm_destruct t1 cs t2) T4
+  | typing_absurd : forall E T1 T2 T3 t1,
+      kinding E T3 knd_type ->
+      typing E t1 (typ_variant T1 T2) ->
+      E ||= T1 -<: (typ_bot cons_universe) ->
+      E ||= T2 -<: T1 ->
       typing E (trm_absurd t1) T3.
 
 Notation "E |= t -: T" := (typing E t T) (at level 69).
 
 Definition typing_scheme E t M :=
+  kinds (sch_arity M) (sch_kinds M) /\
   exists L, forall Xs,
     fresh L (sch_arity M) Xs ->
     (E & Xs ~::* sch_kinds M) |= t -: (M ^ Xs).
@@ -529,18 +759,30 @@ Inductive red : trm -> trm -> Prop :=
       term_body t3 ->
       red t1 t1' ->
       red (trm_match t1 c t2 t3) (trm_match t1' c t2 t3)
-  | red_match_2 : forall c t1 t2 t3,
+  | red_match_2 : forall c cs t1 t2 t3,
+      In c cs ->
       value (trm_constructor c t1) ->
       term_body t2 ->
       term_body t3 ->
-      red (trm_match (trm_constructor c t1) c t2 t3) (t2 ^^ t1)
-  | red_match_3 : forall c d t1 t2 t3,
-      c <> d ->
-      value (trm_constructor d t1) ->
+      red (trm_match (trm_constructor c t1) cs t2 t3)
+          (t2 ^^ (trm_constructor c t1))
+  | red_match_3 : forall c cs t1 t2 t3,
+      ~ In c cs ->
+      value (trm_constructor c t1) ->
       term_body t2 ->
       term_body t3 ->
-      red (trm_match (trm_constructor d t1) c t2 t3)
-          (t3 ^^ (trm_constructor d t1))
+      red (trm_match (trm_constructor c t1) cs t2 t3)
+          (t3 ^^ (trm_constructor c t1))
+  | red_destruct_1 : forall c t1 t1' t2,
+      term_body t2 ->
+      red t1 t1' ->
+      red (trm_destruct t1 c t2) (trm_destruct t1' c t2)
+  | red_destruct_2 : forall c cs t1 t2,
+      In c cs ->
+      value (trm_constructor c t1) ->
+      term_body t2 ->
+      red (trm_destruct (trm_constructor c t1) cs t2)
+          (t2 ^^ t1)
   | red_absurd : forall t1 t1',
       red t1 t1' ->
       red (trm_absurd t1) (trm_absurd t1').
