Infrastructure.v
@@ -6,7 +6,6 @@
 Set Implicit Arguments.
 Require Import List LibLN Definitions.
 
-
 (* =============================================================== *)
 (** * Additional Definitions used in the Proofs *)
 
@@ -20,10 +19,11 @@ Fixpoint typ_fv (T : typ) {struct T} : vars :=
   | typ_bvar i => \{}
   | typ_fvar x => \{x}
   | typ_constructor c T1 => (typ_fv T1)
+  | typ_or T1 T2 => (typ_fv T1) \u (typ_fv T2)
   | typ_variant T1 T2 => (typ_fv T1) \u (typ_fv T2)
   | typ_arrow T1 T2 => (typ_fv T1) \u (typ_fv T2)
-  | typ_top => \{}
-  | typ_bot => \{}
+  | typ_top cs => \{}
+  | typ_bot cs => \{}
   | typ_meet T1 T2 => (typ_fv T1) \u (typ_fv T2)
   | typ_join T1 T2 => (typ_fv T1) \u (typ_fv T2)
   end.
@@ -42,7 +42,7 @@ Definition sch_fv M :=
 
 Definition bind_fv (B : bind) : vars :=
   match B with
-  | bind_kind K => \{}
+  | bind_knd K => \{}
   | bind_typ M => sch_fv M
   end.
 
@@ -60,6 +60,7 @@ Fixpoint trm_fv (t : trm) {struct t} : vars :=
   | trm_app t1 t2 => (trm_fv t1) \u (trm_fv t2)
   | trm_constructor c t1 => trm_fv t1
   | trm_match t1 c t2 t3 => (trm_fv t1) \u (trm_fv t2) \u (trm_fv t3)
+  | trm_destruct t1 c t2 => (trm_fv t1) \u (trm_fv t2)
   | trm_absurd t1 => trm_fv t1
   end.
 
@@ -73,12 +74,14 @@ Fixpoint typ_subst (Z : var) (U : typ) (T : typ) {struct T} : typ :=
   | typ_bvar i => typ_bvar i
   | typ_fvar X => If X = Z then U else (typ_fvar X)
   | typ_constructor c T1 => typ_constructor c (typ_subst Z U T1)
+  | typ_or T1 T2 =>
+      typ_or (typ_subst Z U T1) (typ_subst Z U T2)
   | typ_variant T1 T2 =>
       typ_variant (typ_subst Z U T1) (typ_subst Z U T2)
   | typ_arrow T1 T2 =>
       typ_arrow (typ_subst Z U T1) (typ_subst Z U T2)
-  | typ_top => typ_top
-  | typ_bot => typ_bot
+  | typ_top cs => typ_top cs
+  | typ_bot cs => typ_bot cs
   | typ_meet T1 T2 =>
       typ_meet (typ_subst Z U T1) (typ_subst Z U T2)
   | typ_join T1 T2 =>
@@ -107,10 +110,18 @@ Definition sch_substs Zs Us M :=
 (** Substitution for bindings *)
 Definition binding_subst Z U B :=
   match B with
-  | bind_kind K => bind_kind K
+  | bind_knd K => bind_knd K
   | bind_typ M => bind_typ (sch_subst Z U M)
   end.
 
+Fixpoint binding_substs (Zs : list var) (Us : list typ) (B : bind)
+   {struct Zs} : bind :=
+  match Zs, Us with
+  | Z::Zs', U::Us' => binding_substs Zs' Us' (binding_subst Z U B)
+  | _, _ => B
+  end.
+
+(** Substitution for environments *)
 Definition environment_subst Z U E :=
   map (binding_subst Z U) E.
 
@@ -134,6 +145,8 @@ Fixpoint trm_subst (z : var) (u : trm) (t : trm) {struct t} : trm :=
   | trm_match t1 c t2 t3 =>
       trm_match (trm_subst z u t1) c
                 (trm_subst z u t2) (trm_subst z u t3)
+  | trm_destruct t1 c t2 =>
+      trm_destruct (trm_subst z u t1) c (trm_subst z u t2)
   | trm_absurd t1 => trm_absurd (trm_subst z u t1)
   end.
 
@@ -176,7 +189,7 @@ Tactic Notation "exists_fresh" ident(x) ident(Hfr) :=
 (* *************************************************************** *)
 (** ** Automation *)
 
-Hint Constructors type term environment type_equal kinding kinding_env typing value red.
+Hint Constructors kind type term environment type_equal kinding kinding_env typing value red.
 
 Lemma typ_def_fresh : typ_fv typ_def = \{}.
 Proof.
@@ -188,6 +201,8 @@ Hint Extern 1 (_ \notin typ_fv typ_def) =>
 
 Hint Extern 1 (types _ _) => split; auto.
 
+Hint Extern 1 (kinds _ _) => split; auto.
+
 Hint Extern 1 =>
   match goal with
   | H : forall x, x \notin ?L -> ?P |- ?P =>
@@ -197,6 +212,51 @@ Hint Extern 1 =>
     apply (H (proj1_sig (var_freshes L n))
              (proj2_sig (var_freshes L n)))
   end.
+
+Lemma liblist_length_eq_length : forall A (L : list A),
+    LibList.length L = length L.
+Proof.
+  intros.
+  induction L.
+  - rewrite LibList.length_nil.
+    auto.
+  - rewrite LibList.length_cons.
+    simpl.
+    auto.
+Qed.
+
+Lemma fresh_length_resize : forall L n xs,
+    fresh L n xs -> fresh L (length xs) xs.
+Proof.
+  intros.
+  rewrite <- liblist_length_eq_length.
+  apply fresh_resize_length with n.
+  assumption.
+Qed.
+
+Hint Resolve fresh_length_resize.
+
+Lemma fresh_length_arity : forall L Xs M,
+    fresh L (sch_arity M) Xs ->
+    fresh L (length (sch_kinds M)) Xs.
+Proof.
+  unfold sch_arity.
+  auto.
+Qed.
+
+Hint Resolve fresh_length_arity.
+
+Lemma fresh_length_arity_subst : forall L Xs M X U,
+    fresh L (sch_arity (sch_subst X U M)) Xs ->
+    fresh L (sch_arity M) Xs.
+Proof.
+  unfold sch_arity.
+  unfold sch_subst.
+  simpl.
+  auto.
+Qed.
+
+Hint Resolve fresh_length_arity_subst.
 
 Lemma kinds_nil : forall E,
     E & nil ~::* nil = E.
@@ -270,6 +330,8 @@ Proof.
     apply* (@trm_open_rec_core t2 0 (trm_fvar x)). }
   { unfolds trm_open. pick_fresh x.
     apply* (@trm_open_rec_core t3 0 (trm_fvar x)). }
+  { unfolds trm_open. pick_fresh x.
+    apply* (@trm_open_rec_core t2 0 (trm_fvar x)). }
 Qed.
 
 (** Substitution for a fresh name is identity. *)
@@ -322,6 +384,7 @@ Proof.
   - apply_fresh term_abs as y. rewrite* trm_subst_open_var.
   - apply_fresh* term_let as y. rewrite* trm_subst_open_var.
   - apply_fresh* term_match as y; rewrite* trm_subst_open_var.
+  - apply_fresh* term_destruct as y; rewrite* trm_subst_open_var.
 Qed.
 
 Hint Resolve trm_subst_term.
@@ -372,7 +435,25 @@ Proof.
   apply* (@term_match (x \u x0)).
 Qed.
 
-Hint Resolve body_to_term_abs body_to_term_let bodies_to_term_match.
+Lemma term_destruct_to_body : forall c t1 t2,
+  term (trm_destruct t1 c t2) -> term_body t2.
+Proof.
+  intros. unfold term_body. inversion* H.
+Qed.
+
+Lemma body_to_term_destruct : forall c t1 t2,
+  term t1 -> term_body t2 ->
+  term (trm_destruct t1 c t2).
+Proof.
+  intros. inversion H0.
+  apply* (@term_destruct x).
+Qed.
+
+Hint Resolve
+     body_to_term_abs
+     body_to_term_let
+     bodies_to_term_match
+     body_to_term_destruct.
 
 Hint Extern 1 (term_body ?t) =>
   match goal with 
@@ -527,6 +608,71 @@ Proof.
   intros. apply* (@typ_substs_intro_ind T Xs Us nil).
 Qed.
 
+Lemma typ_substs_intro_sch : forall M Xs Us,
+  fresh (sch_fv M \u typ_fv_list Us) (sch_arity M) Xs -> 
+  types (sch_arity M) Us ->
+  length Xs = sch_arity M ->
+  sch_open M Us = typ_substs Xs Us (sch_open_vars M Xs).
+Proof.
+  introv Hf Ht Hl.
+  apply typ_substs_intro; rewrite Hl; auto.
+Qed.
+
+Lemma sch_subst_no_params : forall X U T,
+    sch_subst X U (Sch nil T) =
+    Sch nil (typ_subst X U T).
+Proof.
+  unfold sch_subst.
+  simpl.
+  reflexivity.
+Qed.
+
+Lemma typ_subst_constructor : forall X U c T,
+  typ_subst X U (typ_constructor c T) =
+  typ_constructor c (typ_subst X U T).
+Proof.
+  auto.
+Qed.
+
+Lemma typ_subst_variant : forall X U T1 T2,
+  typ_subst X U (typ_variant T1 T2) =
+  typ_variant (typ_subst X U T1) (typ_subst X U T2).
+Proof.
+  auto.
+Qed.
+
+Lemma typ_subst_join : forall X U T1 T2,
+  typ_subst X U (typ_join T1 T2) =
+  typ_join (typ_subst X U T1) (typ_subst X U T2).
+Proof.
+  auto.
+Qed.
+
+Lemma typ_subst_or : forall X U T1 T2,
+  typ_subst X U (typ_or T1 T2) =
+  typ_or (typ_subst X U T1) (typ_subst X U T2).
+Proof.
+  auto.
+Qed.
+
+Lemma typ_subst_bot : forall X U cs,
+  typ_subst X U (typ_bot cs) =
+  typ_bot cs.
+Proof.
+  auto.
+Qed.
+
+Lemma typ_subst_row : forall X U cs T R,
+  typ_subst X U (typ_row cs T R) =
+  typ_row cs (typ_subst X U T) (typ_subst X U R).
+Proof.
+  unfold typ_row.
+  intros.
+  induction cs; simpl; auto.
+  rewrite IHcs.
+  easy.
+Qed.
+
 (** Types are stable by type substitution *)
 
 Lemma typ_subst_type : forall T Z U,
@@ -635,10 +781,10 @@ Proof.
   unfold scheme, sch_subst, sch_arity.
   intros Z U [Ks T] TU S.
   simpls.
-  destruct S as [L H].
+  destruct S as [[L H] Hk].
+  split; auto.
   exists_fresh Xs Fr.
-  rewrite* typ_subst_open_vars.
-  rewrite* (fresh_length _ _ _ Fr) in Fr.
+  rewrite typ_subst_open_vars; eauto.
 Qed.
 
 Hint Resolve sch_subst_type.
@@ -658,7 +804,7 @@ Lemma sch_open_types : forall M Us,
   types (sch_arity M) Us ->
   type (sch_open M Us).
 Proof.
-  intros [Ks T] Us Hb [Ha Ht].
+  intros [Ks T] Us [Hb Hk] [Ha Ht].
   simpls. apply* typ_open_types.
 Qed.
 
@@ -674,7 +820,7 @@ Proof.
   introv H.
   inverts H as H1 H2 H3 H4.
   - false (empty_push_inv H1).
-  - destruct (eq_push_inv H3) as [_ [Hv _]].
+  - destruct (eq_push_inv H4) as [_ [Hv _]].
     false Hv.
   - destruct (eq_push_inv H4) as [Hx [Hv He]].
     inversion Hv.
@@ -683,13 +829,14 @@ Proof.
 Qed.
 
 Lemma environment_kind_push_inv : forall E x K,
-    environment (E & x ~ (bind_kind K)) ->
-    environment E /\ x # E.
+    environment (E & x ~ (bind_knd K)) ->
+    environment E /\ x # E /\ kind K.
 Proof.
   introv H.
   inverts H as H1 H2 H3 H4.
   - false (empty_push_inv H1).
-  - destruct (eq_push_inv H3) as [Hx [_ He]].
+  - destruct (eq_push_inv H4) as [Hx [Hk He]].
+    inversion Hk.
     subst.
     easy.
   - destruct (eq_push_inv H4) as [_ [Hv _]].
@@ -711,8 +858,8 @@ Proof.
 Qed.
 
 Lemma environment_kind_middle_inv : forall E x K F,
-    environment (E & x ~ (bind_kind K) & F) ->
-    environment (E & F) /\ x # E.
+    environment (E & x ~ (bind_knd K) & F) ->
+    environment (E & F) /\ x # E /\ kind K.
 Proof.
   introv H.
   induction F using env_ind; rew_env_concat.
@@ -776,7 +923,7 @@ Proof.
   rewrite concat_assoc in *.
   destruct v; simpl.
   - destruct (environment_kind_push_inv He).
-    apply* environment_kind.
+    apply* environment_knd.
   - destruct (environment_typ_push_inv He).
     apply*  environment_typ.
 Qed.
@@ -790,18 +937,82 @@ Proof.
   auto.
 Qed.
 
+Lemma environment_subst_push : forall X T E Y B,
+    environment_subst X T (E & Y ~ B)
+    = environment_subst X T E & Y ~ binding_subst X T B.
+Proof.
+  intros.
+  unfold environment_subst.
+  rewrite map_push.
+  auto.
+Qed.
+
+Lemma dom_environment_subst : forall X T E,
+    dom (environment_subst X T E) = dom E.
+Proof.
+  intros.
+  unfold environment_subst.
+  rewrite dom_map.
+  easy.
+Qed.
+
+Lemma environment_subst_kinds : forall X T E Xs Ks,
+    fresh \{X} (length Ks) Xs ->
+    environment_subst X T (E & Xs ~::* Ks) =
+    environment_subst X T E & Xs ~::* Ks.
+Proof.
+  introv Hf.
+  unfold environment_subst.
+  rewrite map_concat.
+  lets Hlx : (eq_sym (fresh_length _ _ _ Hf)).
+  gen Ks.
+  induction Xs; destruct Ks;
+    introv Hf Hl; tryfalse; auto.
+  - rewrite singles_nil.
+    rewrite! map_empty.
+    easy.
+  - inversion Hl.
+    rewrite singles_cons.
+    rewrite! map_push.
+    simpl binding_subst.
+    rewrite! concat_assoc.
+    rewrite* IHXs.
+    destruct* Hf.
+Qed.   
+    
 Lemma environment_substs_empty : forall Xs Ts,
     length Xs = length Ts ->
     environment_substs Xs Ts empty = empty.
 Proof.
   introv Hl.
   gen Ts.
-  induction Xs.
-  - induction Ts; introv Hl; tryfalse; auto.
-  - induction Ts; introv Hl; tryfalse.
-    simpl.
-    rewrite environment_subst_empty.
-    auto.
+  induction Xs; destruct Ts; intros; tryfalse; auto.
+  simpl.
+  rewrite environment_subst_empty.
+  auto.
+Qed.
+
+Lemma environment_substs_push : forall Xs Ts E Y B,
+    environment_substs Xs Ts (E & Y ~ B)
+    = environment_substs Xs Ts E & Y ~ binding_substs Xs Ts B.
+Proof.
+  intros.
+  gen E Ts B.
+  induction Xs; destruct Ts; intros; tryfalse; auto.
+  simpl.
+  rewrite environment_subst_push.
+  apply IHXs.
+Qed.
+
+Lemma dom_environment_substs : forall Xs Ts E,
+    dom (environment_substs Xs Ts E) = dom E.
+Proof.
+  intros.
+  gen Ts E.
+  induction Xs; destruct Ts; intros; tryfalse; auto.
+  simpl.
+  rewrite IHXs.
+  apply dom_environment_subst.
 Qed.
 
 Lemma fresh_kinds : forall E x n Xs Ks,
@@ -832,6 +1043,7 @@ Lemma environment_kinds : forall E n Xs Ks,
     environment E ->
     (fresh (dom E) n Xs) ->
     length Ks = n ->
+    Forall kind Ks ->
     environment (E & Xs ~::* Ks).
 Proof.
   introv He Hf Hlk.
@@ -839,24 +1051,26 @@ Proof.
   gen Ks n.
   induction Xs; destruct Ks;
     intros; subst; tryfalse; rew_kinds*.
-  apply environment_kind.
-  - eapply IHXs; intuition.
-    destruct* Hf.
+  apply environment_knd.
+  - eapply IHXs; iauto.
+    + destruct* Hf.
+    + inversion H; auto.
+  - inversion H; auto.
   - eapply fresh_kinds; auto.
 Qed.
 
 (** Binding substitution is identity on bind_kind. *)
 
 Lemma binding_subst_kind : forall x T K,
-  binding_subst x T (bind_kind K) = bind_kind K.
+  binding_subst x T (bind_knd K) = bind_knd K.
 Proof.
   simpl.
   reflexivity.
 Qed.
 
 Lemma binds_subst_inv_r : forall E F X Y T K,
-    binds X (bind_kind K) (E & F) ->
-    binds X (bind_kind K) (E & environment_subst Y T F).
+    binds X (bind_knd K) (E & F) ->
+    binds X (bind_knd K) (E & environment_subst Y T F).
 Proof.
   introv H.
   unfolds environment_subst.
@@ -868,7 +1082,31 @@ Proof.
 Qed.
 
 Hint Resolve binds_subst_inv_r.
-    
+
+Lemma binds_environment_subst : forall E F X T K x M,
+    binds x (bind_typ M) (E & X ~:: K & F) ->
+    X \notin (env_fv E) ->
+    binds x (bind_typ (sch_subst X T M))
+          (E & environment_subst X T F).
+Proof.
+  introv Hb Hn.
+  destruct (binds_concat_inv Hb) as [Hbf | [Hf Hbex]].
+  - apply binds_concat_right.
+    unfold environment_subst.
+    fold (binding_subst X T (bind_typ M)).
+    apply* binds_map.
+  - apply binds_concat_left.
+    + { destruct (binds_concat_inv Hbex) as [Hbx | [_ Hbe]].
+        - destruct (binds_single_inv Hbx).
+          tryfalse.
+        - rewrite* sch_subst_fresh.
+          fold (bind_fv (bind_typ M)).
+          apply fv_in_values_binds with (x := x) (E := E); auto. }
+    + rewrite* dom_environment_subst.
+Qed.
+
+Hint Resolve binds_environment_subst.
+
 Lemma ok_from_environment : forall E,
   environment E -> ok E.
 Proof.
@@ -899,6 +1137,493 @@ Proof.
     + eapply IHE; auto.
 Qed.
 
+Lemma kind_from_env : forall E x K,
+    environment E ->
+    binds x (bind_knd K) E ->
+    kind K.
+Proof.
+  introv He Hb.
+  induction E using env_ind; rew_env_concat.
+  - false (binds_empty_inv Hb).
+  - destruct (binds_push_inv Hb)
+      as [ [ Hvar Hbind ] | [ Hvar Hbind ] ].
+    + { subst.
+        inversion He.
+        - false (empty_push_inv H0).
+        - destruct (eq_push_inv H) as [_ [Heq _]].
+          inversion Heq.
+          subst*.
+        - destruct (eq_push_inv H) as [_ [Heq _]].
+          false Heq. }
+    + eapply IHE; auto.
+Qed.
+
+Lemma kinds_from_env : forall E Xs Ks,
+    environment (E & Xs ~::* Ks) ->
+    length Xs = length Ks ->
+    kinds (length Ks) Ks.
+Proof.
+  introv He Hl.
+  split*.
+  gen Xs.
+  induction Ks; introv He Hl; auto.
+  destruct Xs; tryfalse.
+  rew_kinds in He.
+  inversion He.
+  - apply empty_push_inv in H0.
+    tryfalse.
+  - destruct (eq_push_inv H) as [? [Hb ?]].
+    inversion Hb.
+    inversion Hl.
+    subst.
+    eauto.
+  - destruct (eq_push_inv H) as [_ [Hb _]].
+    tryfalse.
+Qed.
+
+Lemma env_fv_empty :
+  env_fv empty = \{}.
+Proof.
+  unfold env_fv, fv_in_values.
+  rew_env_defs.
+  simpl.
+  auto.
+Qed.
+
+Lemma env_fv_push_inv : forall E X B,
+    env_fv (E & X ~ B) = bind_fv B \u env_fv E.
+Proof.
+  intros.
+  unfold env_fv, fv_in_values.
+  rewrite values_def.
+  rewrite <- cons_to_push.
+  rewrite LibList.map_cons.
+  simpl.
+  auto.
+Qed.
+
+(** Substitution for a fresh name is identity. *)
+
+Lemma binding_subst_fresh : forall X U B, 
+  X \notin bind_fv B -> 
+  binding_subst X U B = B.
+Proof.
+  intros.
+  destruct B; simpl; auto.
+  f_equal.
+  simpl in H.
+  apply sch_subst_fresh.
+  assumption.
+Qed.
+
+Lemma binding_substs_fresh : forall Xs Us B, 
+  fresh (bind_fv B) (length Xs) Xs ->
+  binding_substs Xs Us B = B.
+Proof.
+  intros.
+  gen Us.
+  induction Xs; intros; auto.
+  destruct Us; auto.
+  simpl in H.
+  simpl.
+  rewrite* binding_subst_fresh.
+Qed.
+
+Lemma environment_subst_fresh : forall X U E, 
+  X \notin env_fv E -> 
+  environment_subst X U E = E.
+Proof.
+  intros.
+  unfold environment_subst.
+  induction E using env_ind.
+  - rewrite* map_empty.
+  - rewrite env_fv_push_inv in H.
+    rewrite notin_union in H.
+    rewrite map_push.
+    rewrite* binding_subst_fresh.
+    rewrite* IHE.
+Qed.
+
+Lemma environment_substs_fresh : forall Xs Us E, 
+  fresh (env_fv E) (length Xs) Xs ->
+  environment_substs Xs Us E = E.
+Proof.
+  intros.
+  gen Us.
+  induction Xs; intros; auto.
+  destruct Us; auto.
+  simpl in H.
+  simpl.
+  rewrite* environment_subst_fresh.
+Qed.
+
+Hint Rewrite in_empty in_singleton in_union : rew_in.
+
+Tactic Notation "rew_in" :=
+  autorewrite with rew_in.
+
+Tactic Notation "rew_in" "in" hyp(H) :=
+  autorewrite with rew_in in H.
+
+Lemma typ_fv_open_vars : forall T Xs X,
+    X \in typ_fv T ->
+    X \in typ_fv (typ_open_vars T Xs).
+Proof.
+  introv Hfv.
+  unfold typ_open_vars, typ_fvars.
+  induction T;
+    simpl; simpl in Hfv; rew_in; rew_in in Hfv; iauto.
+Qed.
+
+Lemma kinding_closed : forall E T K X,
+    kinding E T K ->
+    X \in typ_fv T ->
+    X \in dom E.
+Proof.
+  introv Hk Hfv.
+  induction Hk; simpl in Hfv; rew_in in Hfv; iauto.
+  subst.
+  eapply get_some_inv.
+  apply H0.
+Qed.
+
+Lemma kinding_scheme_closed : forall E M X,
+    kinding_scheme E M ->
+    X \in sch_fv M ->
+    X \in dom E.
+Proof.
+  introv Hks Hfv.
+  unfold kinding_scheme, kinding_body in Hks.
+  unfold sch_fv in Hfv.
+  destruct Hks as [L Hk].
+  pick_freshes (sch_arity M) Xs.
+  destruct Hk with Xs as [_ Hkk]; auto.
+  eapply kinding_closed with (X := X) in Hkk; auto.
+  - rewrite dom_concat in Hkk.
+    rew_in in Hkk.
+    destruct* Hkk.
+    rewrite dom_map in H.
+    rewrite dom_singles in H.
+    + assert (fresh \{X} (sch_arity M) Xs) by auto.
+      eapply fresh_single_notin in H; auto.
+      tryfalse.
+    + apply fresh_length in Fr.
+      unfold sch_arity in Fr.
+      rewrite! liblist_length_eq_length.
+      auto.
+  - apply* typ_fv_open_vars.
+Qed.
+
+Lemma kinding_env_closed : forall E X,
+    kinding_env E ->
+    X \in env_fv E ->
+    X \in dom E.
+Proof.
+  introv Hk Hfv.
+  induction Hk.
+  - rewrite env_fv_empty in Hfv.
+    rew_in in Hfv.
+    iauto.
+  - rewrite env_fv_push_inv in Hfv.
+    rewrite dom_push.
+    rew_in.
+    right.
+    rew_in in Hfv.
+    destruct* Hfv.
+  - rewrite env_fv_push_inv in Hfv.
+    rewrite dom_push.
+    rew_in.
+    right.
+    rew_in in Hfv.
+    destruct* Hfv.
+    simpl in H1.
+    apply kinding_scheme_closed with M; auto.
+Qed.
+
+(* =============================================================== *)
+(** ** Automation for fset and constructors *)
+
+Lemma fset_from_list_mem : forall A (x : A) L,
+  x \in from_list L = LibList.Mem x L.
+Proof using.
+  unfold from_list. induction L; simpl.
+  - rewrite in_empty.
+    rewrite LibList.Mem_nil_eq.
+    reflexivity.
+  - rewrite in_union.
+    rewrite in_singleton.
+    rewrite~ LibList.Mem_cons_eq.
+    congruence.
+Qed.
+
+Lemma fset_in_decidable : forall (A : fset nat) x,
+    x \in A \/ x \notin A.
+Proof.
+  unfold notin.
+  intros.
+  destruct (fset_finite A) as [l].
+  subst.
+  rewrite fset_from_list_mem.
+  assert ((LibList.Mem x l /\ LibReflect.decide (LibList.Mem x l) = true)
+          \/ (~ (LibList.Mem x l) /\ LibReflect.decide (LibList.Mem x l) = false))
+    by apply LibReflect.decide_cases.
+  iauto.
+Qed.
+
+Lemma notin_remove_nat : forall (x : nat) E F,
+  x \notin (E \- F) <-> (x \notin E) \/ (x \in F).
+Proof.
+  intros. unfold notin. rewrite* in_remove.
+  destruct (fset_in_decidable E x);
+  destruct (fset_in_decidable F x);
+  unfold notin;
+  iauto.
+Qed.
+
+Lemma notin_empty : forall A (x : A),
+    x \notin \{} = True.
+Proof.
+  intros.
+  unfold notin.
+  rewrite in_empty.
+  auto.
+Qed.
+
+Hint Rewrite in_empty : rew_fset.
+Hint Rewrite in_union : rew_fset.
+Hint Rewrite in_inter : rew_fset.
+Hint Rewrite in_remove : rew_fset.
+Hint Rewrite notin_empty : rew_fset.
+Hint Rewrite notin_union : rew_fset.
+Hint Rewrite notin_remove_nat : rew_fset.
+
+Lemma fset_extens_inv : forall A (E : fset A) F x,
+    E = F ->
+    (x \in E -> x \in F)
+    /\ (x \in F -> x \in E).
+Proof.
+  intros. subst. iauto.
+Qed.
+
+Ltac inList x xs :=
+  match xs with
+    | tt => constr:false
+    | (x, _) => constr:true
+    | (_, ?xs') => inList x xs'
+  end.
+
+Ltac fsets_decide_all v xs :=
+  try match goal with
+  | [ x : fset nat |- _ ] =>
+    let b := inList x xs in
+    match b with
+    | true => fail 1
+    | false =>
+      try fsets_decide_all v (x, xs);
+      let dec := fresh "decidable" in
+      destruct (fset_in_decidable x v) as [dec | dec];
+      unfold notin in dec
+    end
+  end.
+
+Ltac fsets_abstract_singleton v :=
+  let single := fresh "single" in
+  let Heq_single := fresh "Heq_single" in
+  remember \{v} as single eqn:Heq_single;
+  let Heq_v := fresh "Heq_v" in
+  assert (forall S, v \in S -> subset single S)
+    by ( intros; unfold subset; intro;
+         rewrite Heq_single; rewrite in_singleton;
+         intro Heq_v; rewrite Heq_v; assumption );
+  let Hin := fresh "Hin" in
+  assert (forall S, v \notin S -> disjoint single S)
+    by ( intro; unfold notin; unfold disjoint; rewrite Heq_single;
+         intro; apply fset_extens;
+         unfold subset; intro; rewrite in_empty;
+         intro Hin; tryfalse; rewrite in_inter in Hin;
+         rewrite in_singleton in Hin; destruct Hin;
+         tryfalse );
+  assert (v \in single)
+    by ( rewrite Heq_single;
+         rewrite in_singleton;
+         reflexivity ).
+
+Ltac fsets_core :=
+  repeat
+    match goal with
+    | [ |- context[\{?v}] ] =>
+      fsets_abstract_singleton v
+    end;
+  repeat
+    match goal with
+    | [ H : exists x, x \in ?S |- _] =>
+      destruct H
+    end;
+  try unfold subset in *;
+  match goal with
+  | [ |- forall (_ : ?A), _ \in _ -> _ \in _ ] =>
+    let fresh_x := fresh "x" in
+    intro fresh_x;
+    repeat
+      match goal with
+      | [ H : ?S3 = ?S4 |- _ ] =>
+        apply fset_extens_inv with (x := fresh_x) in H;
+        autorewrite with rew_fset in H
+      | [ H : forall (_ : A), _ \in _ -> _ \in _ |- _ ] =>
+        specialize (H fresh_x);
+        autorewrite with rew_fset in H
+      end;
+    autorewrite with rew_fset;
+    fsets_decide_all fresh_x tt;
+    unfold notin;
+    intuition eauto;
+    tryfalse
+  | [ |- ?S1 = ?S2 ] =>
+    apply fset_extens;
+    fsets_core
+  | [ |- exists x, x \in ?S ] =>
+    econstructor;
+    autorewrite with rew_fset;
+    unfold notin;
+    intuition eauto;
+    tryfalse
+  | [ H : ?y \in _ |- False ] =>
+    let A := type of y in
+    repeat
+      match goal with
+      | [ H : ?S3 = ?S4 |- _ ] =>
+        apply fset_extens_inv with (x := y) in H;
+        autorewrite with rew_fset in H
+      | [ H : forall (_ : A), _ \in _ -> _ \in _ |- _ ] =>
+        specialize (H y);
+        autorewrite with rew_fset in H
+      end;
+      autorewrite with rew_fset in H;
+      fsets_decide_all y tt;
+      unfold notin in H;
+      solve [intuition eauto]
+  end.
+
+Ltac fsets_get E :=
+  match E with
+  | context [?cs] =>
+    match type of cs with
+    | fset _ => cs
+    end
+  end.
+
+Ltac fsets :=
+  try unfold disjoint in *;
+  match goal with
+  | [ |- (subset _ _) ] =>
+    solve [ fsets_core ]
+  | [ |- exists x, x \in ?A ] =>
+    solve [ fsets_core ]
+  | [ |- ?A = ?B] =>
+    let cs := fsets_get A in
+    let ds := fsets_get B in
+    let Heq := fresh "Heq" in
+    assert (cs = ds) as Heq by fsets_core;
+    rewrite Heq at 1;
+    reflexivity
+  | [ |- ?A -> ?B ] =>
+    let cs := fsets_get A in
+    let ds := fsets_get B in
+    let Heq := fresh "Heq" in
+    assert (cs = ds) as Heq by fsets_core;
+    rewrite Heq at 1;
+    intro;
+    assumption
+  | [ |- False ] =>
+    fsets_core
+  | [ H : ?A |- ?B ] =>
+    let cs := fsets_get A in
+    let ds := fsets_get B in
+    let Heq := fresh "Heq" in
+    assert (cs = ds) as Heq by fsets_core;
+    rewrite Heq in H at 1;
+    assumption
+  end.
+
+Hint Extern 2 => fsets : fsets.
+
+Ltac constrs :=
+  unfold cons_universe in *;
+  repeat
+    match goal with
+    | [ C : constructors |- _ ] =>
+      destruct C
+    | _ => fail 1
+    end;
+  simpl cons_disjoint in *;
+  simpl cons_union in *;
+  simpl cons_inter in *;
+  simpl cons_subset in *;
+  simpl cons_diff in *;
+  simpl cons_non_empty in *;
+  iauto;
+  fsets.
+
+Hint Extern 2 => constrs : constrs.
+
+Lemma cons_union_commutative : forall cs1 cs2,
+    cons_union cs1 cs2 = cons_union cs2 cs1.
+Proof.
+  intros.
+  constrs.
+Qed.
+
+Lemma cons_union_associative : forall cs1 cs2 cs3,
+    cons_union cs1 (cons_union cs2 cs3)
+    = cons_union (cons_union cs1 cs2) cs3.
+Proof.
+  intros.
+  constrs.
+Qed.
+
+Lemma cons_union_universe : forall cs,
+    cons_union (cons_finite cs) (cons_cofinite cs)
+    = cons_universe.
+Proof.
+  intros.
+  constrs.
+Qed.
+
+Lemma cons_diff_union : forall cs1 cs2,
+    cons_disjoint cs1 cs2 ->
+    cons_diff (cons_union cs1 cs2) cs2 = cs1.
+Proof.
+  intros.
+  constrs.
+Qed.
+
+Lemma cons_diff_universe_cofinite : forall cs,
+    cons_diff cons_universe (cons_cofinite cs)
+    = cons_finite cs.
+Proof.
+  intros.
+  constrs.
+Qed.
+
+Lemma cons_diff_universe_finite : forall cs,
+    cons_diff cons_universe (cons_finite cs)
+    = cons_cofinite cs.
+Proof.
+  intros.
+  constrs.
+Qed.
+
+Lemma cons_non_empty_kind : forall cs,
+    kind (knd_row cs) ->
+    cons_non_empty cs.
+Proof.
+  introv Hkd.
+  inversion Hkd.
+  auto.
+Qed.
+
+Hint Resolve cons_non_empty_kind.
+
 (* =============================================================== *)
 (** * Properties of judgments *)
 
@@ -908,45 +1633,71 @@ Qed.
 (** A kinding relation is restricted to well-formed objects. *)
 
 Lemma kinding_regular : forall E T K,
-  kinding E T K -> environment E /\ type T.
+  kinding E T K -> environment E /\ type T /\ kind K.
 Proof.
-  split; induction* H.
+  split; induction H;
+    intuition eauto using kind_from_env with constrs.
+  - inversion H3.
+    inversion H5.
+    auto with constrs.
 Qed.
 
 Lemma kindings_regular : forall E n Ts Ks,
-  kindings E n Ts Ks -> environment E /\ types n Ts.
+  kindings E n Ts Ks ->
+  environment E /\ types n Ts /\ kinds n Ks.
 Proof.
   split; induction* H.
   split.
-  - simpl.
-    f_equal.
-    destruct* IHkindings.
-  - lets [_ Ht] : (kinding_regular H).
-    lets [_ Hts] : IHkindings.
-    apply* Forall_cons.
+  - split.
+    + simpl.
+      f_equal.
+      destruct IHkindings as [[Hl Ht] Hk]; auto.
+    + lets [_ [Ht Hk]] : (kinding_regular H).
+      lets [[_ Hts] Hks] : IHkindings.
+      apply* Forall_cons.
+  - split.
+    + simpl.
+      f_equal.
+      destruct IHkindings as [_ [Hl Hks]]; auto.
+    + destruct IHkindings as [_ [Hl Hks]]; auto.
+      lets [_ [Ht Hk]] : (kinding_regular H).
+      apply* Forall_cons.
 Qed.  
+
+Lemma kindings_length : forall E n Ts Ks,
+    kindings E n Ts Ks ->
+    length Ts = n /\ length Ks = n.
+Proof.
+  intros.
+  induction H; simpl; iauto.
+Qed.
 
 Lemma kinding_body_regular : forall E n Ks T,
     kinding_body E n Ks T ->
-    environment E /\ type_body n T.
+    environment E /\ kinds n Ks /\ type_body n T.
 Proof.
   introv H.
   destruct H as [L H].
-  split.
+  splits.
   - pick_freshes n Xs.
-    eapply kinding_regular in H; auto.
-    destruct* H.
+    destruct H with Xs as [_ Hk]; auto.
+    eapply kinding_regular in Hk; auto.
+    destruct* Hk.
+  - pick_freshes n Xs.
+    destruct H with Xs as [Hkd _]; auto.
   - exists_fresh Xs Hf.
-    eapply kinding_regular in H; auto.
-    destruct* H.
+    destruct H with Xs as [_ Hk]; auto.
+    eapply kinding_regular in Hk; auto.
+    destruct* Hk.
 Qed.
 
 Lemma kinding_scheme_regular : forall E M,
     kinding_scheme E M -> environment E /\ scheme M.
 Proof.
-  introv H.
-  destruct (kinding_body_regular H).
-  split*.
+  introv Hks.
+  destruct (kinding_body_regular Hks) as [He [Hk Ht]].
+  split; auto.
+  split; auto.
 Qed.
 
 Lemma kinding_env_regular : forall E,
@@ -955,17 +1706,26 @@ Proof.
   introv H.
   induction* H.
   apply* environment_typ.
-  eapply proj2.
-  apply kinding_scheme_regular.
-  apply H0.
+  apply kinding_scheme_regular in H0.
+  iauto.
 Qed.
 
 (* Automation of kinding regularity lemmas *)
 
+Hint Extern 1 (kind ?K) =>
+  match goal with
+  | H : kinding _ _ K |- _ =>
+      apply (proj33 (kinding_regular H))
+  | H1 : environment ?E, H2 : binds _ (bind_knd K) ?E |- _ =>
+      apply (kind_from_env H1 H2)
+  | H1 : kinding_env ?E, H2 : binds _ (bind_knd K) ?E |- _ =>
+      apply (kind_from_env (kinding_env_regular H1) H2)
+  end.
+
 Hint Extern 1 (type ?T) =>
   match goal with
   | H: kinding _ T _ |- _ =>
-      apply (proj2 (kinding_regular H))
+      apply (proj32 (kinding_regular H))
   end.
 
 Hint Extern 1 (scheme ?M) =>
@@ -983,11 +1743,11 @@ Hint Extern 1 (environment ?E) =>
   | H: kinding_env E |- _ =>
       apply (kinding_env_regular H)
   | H: kinding E _ _ |- _ =>
-      apply (proj1 (kinding_regular H))
+      apply (proj31 (kinding_regular H))
   | H: kindings E _ _ _ |- _ =>
-      apply (proj1 (kindings_regular H))
+      apply (proj31 (kindings_regular H))
   | H: kinding_body E _ _ _ |- _ =>
-      apply (proj1 (kinding_body_regular H))
+      apply (proj31 (kinding_body_regular H))
   | H: kinding_scheme E _ |- _ =>
       apply (proj1 (kinding_scheme_regular H))
   end.
@@ -998,43 +1758,88 @@ Hint Extern 1 (environment (?E & ?F)) =>
       apply (environment_concat_inv H)
   end.
 
+Hint Extern 1 (kinds ?n ?Ks) =>
+  match goal with
+  | H: kindings _ n _ Ks |- _ =>
+      apply (proj33 (kindings_regular H))
+  | H : kinding_body _ n Ks _ |- _ =>
+      apply (proj32 (kinding_body_regular H))
+  end.
+
 Hint Extern 1 (types ?n ?Ts) =>
   match goal with
   | H: kindings _ n Ts _ |- _ =>
-      apply (proj2 (kindings_regular H))
+      apply (proj32 (kindings_regular H))
   end.
 
 Hint Extern 1 (type_body ?n ?T) =>
   match goal with
   | H: kinding_body _ n _ T |- _ =>
-      apply (proj2 (kinding_body_regular H))
+      apply (proj33 (kinding_body_regular H))
+  end.
+
+Ltac invert_all_kinds Hs :=
+  try match goal with
+  | [ H : kind (knd_row _) |- _ ] =>
+    let b := inList H Hs in
+    match b with
+    | true => fail 1
+    | false =>
+      try invert_all_kinds (H, Hs);
+      inversion H
+    end
+  | [ H : kinding _ _ (knd_row ?cs) |- _ ] =>
+    let b := inList H Hs in
+    match b with
+    | true => fail 1
+    | false =>
+      try invert_all_kinds (H, Hs);
+      let Hk := fresh "Hk" in
+      assert (kind (knd_row cs))
+        as Hk by (apply (proj33 (kinding_regular H)));
+      inversion Hk
+    end
+  end.
+
+Ltac kinds :=
+  match goal with
+  | [ |- kind (knd_row _) ] =>
+    invert_all_kinds tt;
+    subst; apply kind_row; constrs
   end.
 
 (** Type equality preserves regularity *)
 
 Lemma type_equal_regular : forall E T1 T2 K,
-    type_equal E T1 T2 K -> environment E /\ type T1 /\ type T2.
+    type_equal E T1 T2 K ->
+    environment E /\ type T1 /\ type T2 /\ kind K.
 Proof.
   introv Ht.
-  induction* Ht. 
+  induction Ht; intuition auto; try kinds.
 Qed.
 
 Lemma subtype_regular : forall E T1 T2,
     subtype E T1 T2 -> environment E /\ type T1 /\ type T2.
 Proof.
   introv Hs.
-  destruct (type_equal_regular Hs) as [ He [ _ Ht ] ].
+  destruct (type_equal_regular Hs) as [ He [ _ [ Ht Hk ] ] ].
   inversion* Ht.
 Qed.
 
 (* Automation of equality regularity lemmas *)
 
+Hint Extern 1 (kind ?K) =>
+  match goal with
+  | H : type_equal _ _ _ K |- _ =>
+      apply (proj44 (type_equal_regular H))
+  end.
+
 Hint Extern 1 (type ?T) =>
   match goal with
   | H: type_equal _ T _ _ |- _ =>
-      apply (proj32 (type_equal_regular H))
+      apply (proj42 (type_equal_regular H))
   | H: type_equal _ _ T _ |- _ =>
-      apply (proj33 (type_equal_regular H))
+      apply (proj43 (type_equal_regular H))
   | H: subtype _ T _ |- _ =>
       apply (proj32 (subtype_regular H))
   | H: subtype _ _ T |- _ =>
@@ -1044,7 +1849,7 @@ Hint Extern 1 (type ?T) =>
 Hint Extern 1 (environment ?E) =>
   match goal with
   | H: type_equal E _ _ _ |- _ =>
-      apply (proj31 (type_equal_regular H))
+      apply (proj41 (type_equal_regular H))
   | H: subtype E _ _ |- _ =>
       apply (proj31 (subtype_regular H))
   end.
@@ -1054,11 +1859,11 @@ Hint Extern 1 (environment (?E & environment_subst ?X ?T ?F)) =>
   | H1: environment (E & X ~:: ?K & F), H2: kinding E T ?K |- _ =>
       apply (environment_subst_inv_r X
                (environment_concat_inv H1)
-               (proj2 (kinding_regular H2)))
+               (proj32 (kinding_regular H2)))
   | H1: environment (E & X ~:: ?K & F), H2: type_equal E T T ?K |- _ =>
       apply (environment_subst_inv_r X
                (environment_concat_inv H1)
-               (proj31 (type_equal_regular H2)))
+               (proj41 (type_equal_regular H2)))
   | H1: environment (E & X ~:: _ & F), H2: type T |- _ =>
       apply (environment_subst_inv_r X (environment_concat_inv H1) H2)
   | H1: environment (E & F), H2: type T |- _ =>
@@ -1080,24 +1885,52 @@ Proof.
     inversion* IHtyping1.
 Qed.
 
+Lemma typing_scheme_regular : forall E e M,
+    typing_scheme E e M -> environment E /\ term e /\ scheme M.
+Proof.
+  unfold typing_scheme.
+  introv [Hks [L Ht]].
+  splits*.
+  - pick_freshes (sch_arity M) Xs.
+    eapply typing_regular in Ht; auto.
+    eapply environment_concat_inv_l; iauto.
+  - pick_freshes (sch_arity M) Xs.
+    eapply typing_regular in Ht; iauto.
+  - unfold scheme, type_body.
+    split*.
+    exists L.
+    introv Hf.
+    eapply typing_regular in Ht; iauto.
+Qed.
+
 (** Automation of typing regularity lemma *)
 
 Hint Extern 1 (environment ?E) =>
   match goal with
   | H: typing E _ _ |- _ =>
       apply (proj31 (typing_regular H))
+  | H: typing_scheme E _ _ |- _ =>
+      apply (proj31 (typing_scheme_regular H))
   end.
 
 Hint Extern 1 (term ?e) =>
   match goal with
   | H: typing _ e _ |- _ =>
       apply (proj32 (typing_regular H))
+  | H: typing_scheme _ e _ |- _ =>
+      apply (proj32 (typing_scheme_regular H))
   end.
 
 Hint Extern 1 (type ?T) =>
   match goal with
   | H: typing _ _ T |- _ =>
       apply (proj33 (typing_regular H))
+  end.
+
+Hint Extern 1 (scheme ?M) =>
+  match goal with
+  | H: typing_scheme _ _ M |- _ =>
+      apply (proj33 (typing_scheme_regular H))
   end.
 
 (** The value predicate is restricted to well-formed terms. *)
@@ -1117,8 +1950,8 @@ Lemma red_regular : forall e e',
   red e e' -> term e /\ term e'.
 Proof.
   introv Hr.
-  induction* Hr.
-  inversion* H.    
+  induction Hr; iauto.
+  inversion* H0.
 Qed.
 
 Hint Extern 1 (term ?t) =>
