Soundness.v
@@ -12,7 +12,7 @@ Require Import LibLN Definitions Infrastructure.
 (* *************************************************************** *)
 (** Weakening *)
 
-Hint Resolve binds_weaken.
+Hint Resolve binds_weaken : weaken.
 
 Lemma kinding_weakening : forall E F G T K,
    kinding (E & G) T K -> 
@@ -20,10 +20,10 @@ Lemma kinding_weakening : forall E F G T K,
    kinding (E & F & G) T K.
 Proof.
   introv Hk He.
-  inductions Hk; auto.
+  inductions Hk; auto with weaken.
 Qed.
 
-Hint Resolve kinding_weakening.
+Hint Resolve kinding_weakening : weaken.
 
 Lemma kinding_weakening_l : forall E F T K,
     kinding E T K ->
@@ -37,7 +37,7 @@ Proof.
   apply* kinding_weakening.
 Qed.
 
-Hint Resolve kinding_weakening_l.
+Hint Resolve kinding_weakening_l : weaken.
 
 Lemma kinding_weakening_r : forall E F T K,
     kinding E T K ->
@@ -50,7 +50,7 @@ Proof.
   apply* kinding_weakening.
 Qed.
 
-Hint Resolve kinding_weakening_r.
+Hint Resolve kinding_weakening_r : weaken.
 
 Lemma kindings_weakening : forall E F G n Ts Ks,
    kindings (E & G) n Ts Ks -> 
@@ -60,11 +60,11 @@ Proof.
   introv Hk He.
   gen_eq EG : (E & G).
   induction Hk; intro; subst; auto.
-  - apply* kindings_nil.
-  - apply* kindings_cons.
+  - apply kindings_nil; auto.
+  - apply kindings_cons; auto with weaken.
 Qed.
 
-Hint Resolve kindings_weakening.
+Hint Resolve kindings_weakening : weaken.
 
 Lemma kinding_body_weakening : forall E F G n Ks T,
     kinding_body (E & G) n Ks T ->
@@ -72,17 +72,21 @@ Lemma kinding_body_weakening : forall E F G n Ks T,
     environment (E & F & G) ->
     kinding_body (E & F & G) n Ks T.
 Proof.
-  unfold kinding_body.
   introv Hk He.
+  destruct (kinding_body_regular Hk) as [_ [Hkd _]].
+  unfold kinding_body in *.
   destruct Hk as [L Hk].
   exists_fresh Xs Hf.
-  apply_ih_bind* kinding_weakening.
-  apply environment_kinds with n; auto.
-  rewrite! dom_concat.
-  auto.
-Qed.  
+  split; auto.
+  apply_ih_bind kinding_weakening.
+  - apply Hk; auto.
+  - apply environment_kinds with n; auto.
+    + rewrite! dom_concat.
+      auto.
+    + destruct Hkd; auto.
+Qed.
 
-Hint Resolve kinding_body_weakening.
+Hint Resolve kinding_body_weakening : weaken.
 
 Lemma kinding_scheme_weakening : forall E F G M,
     kinding_scheme (E & G) M ->
@@ -94,7 +98,7 @@ Proof.
   apply* kinding_body_weakening.
 Qed.
 
-Hint Resolve kinding_scheme_weakening.
+Hint Resolve kinding_scheme_weakening : weaken.
 
 Lemma kinding_scheme_weakening_l : forall E F M,
     kinding_scheme E M ->
@@ -108,21 +112,65 @@ Proof.
   apply* kinding_scheme_weakening.
 Qed.  
 
-Hint Resolve kinding_scheme_weakening_l.
+Hint Resolve kinding_scheme_weakening_l : weaken.
 
 (* *************************************************************** *)
 (** Not affected by type bindings *)
 
-Lemma kinding_bind_typ : forall E T K x S,
+Lemma kinding_bind_typ : forall E F T K x S,
+    kinding (E & x ~: S & F) T K ->
+    kinding (E & F) T K.
+Proof.
+  introv Hk.
+  gen_eq Ex : (E & x ~: S & F).
+  induction Hk; intro; subst; eauto.
+  destruct (binds_middle_inv H0) as [|[[_[_ Heq]]|]]; iauto.
+  inversion Heq.
+Qed.
+
+Lemma kinding_bind_typ_l : forall E T K x S,
     kinding (E & x ~: S) T K ->
     kinding E T K.
 Proof.
   introv Hk.
-  gen_eq Ex : (E & x ~: S).
-  induction Hk; intro; subst; eauto.
-  destruct* (binds_push_inv H0) as [ [ _ Heq ] | ].
-  inversion Heq.
+  rewrite <- concat_empty_r with (E := E).
+  apply kinding_bind_typ with (x := x) (S := S).
+  rewrite concat_empty_r.
+  auto.
 Qed.
+
+Lemma kindings_bind_typ : forall E F n T K x S,
+    kindings (E & x ~: S & F) n T K ->
+    kindings (E & F) n T K.
+Proof.
+  introv Hk.
+  gen_eq G : (E & x ~: S & F).
+  induction Hk; intros; subst.
+  - apply* kindings_nil.
+  - apply* kindings_cons.
+    apply kinding_bind_typ with (x := x) (S := S).
+    auto.
+Qed.
+
+Lemma kinding_scheme_bind_typ : forall E F M x S,
+    kinding_scheme (E & x ~: S & F) M ->
+    kinding_scheme (E & F) M.
+Proof.
+  unfold kinding_scheme, kinding_body.
+  introv [L Hk].
+  exists_fresh Xs HFr.
+  destruct Hk with Xs as [Hkd Hks]; auto.
+  split; auto.
+  rewrite <- concat_assoc.
+  apply kinding_bind_typ with (x := x) (S := S).
+  rewrite concat_assoc.
+  auto.
+Qed.
+
+Hint Resolve kinding_bind_typ : bind_typ.
+Hint Resolve kinding_bind_typ_l : bind_typ.
+Hint Resolve kindings_bind_typ : bind_typ.
+Hint Resolve kinding_scheme_bind_typ : bind_typ.
 
 (* *************************************************************** *)
 (** Preserved by type substitution *)
@@ -196,10 +244,100 @@ Proof.
   - subst*.
 Qed.
 
-Hint Resolve kinding_typ_subst.
+Lemma kindings_typ_subst : forall n E F X Ts S Ks J,
+  kindings (E & X ~:: J & F) n Ts Ks -> 
+  kinding E S J -> 
+  kindings (E & (environment_subst X S F)) n
+           (List.map (typ_subst X S) Ts) Ks.
+Proof.
+  introv Hks Hk.
+  gen_eq G : (E & X ~:: J & F).
+  induction Hks; intro; subst; simpl.
+  - apply kindings_nil.
+    destruct* (environment_kind_middle_inv H).
+  - apply kindings_cons; auto.
+    apply kinding_typ_subst with J; auto.
+Qed.
+
+Lemma kinding_scheme_typ_subst : forall E F M X T K,
+    kinding_scheme (E & X ~:: K & F) M ->
+    kinding E T K ->
+    kinding_scheme (E & environment_subst X T F) (sch_subst X T M).
+Proof.
+  unfold kinding_scheme, kinding_body.
+  introv [L Hs] Ht.
+  exists_fresh Xs Hf.
+  unfold sch_arity in Hf.
+  lets Hlx : (fresh_length _ _ _ Hf).
+  lets Hf2 : Hf.
+  rewrite Hlx in Hf2.
+  apply fresh_length_arity_subst in Hf.
+  destruct Hs with Xs as [Hkd Hks]; auto.
+  split; auto.
+  rewrite <- concat_assoc.
+  rewrite* <- environment_subst_kinds.
+  fold (sch_open_vars (sch_subst X T M) Xs).
+  rewrite* <- sch_subst_open_vars.
+  unfold sch_open_vars.
+  apply kinding_typ_subst with (J := K); auto.
+  rewrite concat_assoc.
+  unfold sch_subst.
+  simpl.
+  apply Hs.
+  unfold sch_arity.
+  unfold sch_subst in Hf.
+  simpl in Hf.
+  auto.
+Qed.
+
+Hint Resolve kinding_typ_subst : typ_subst.
+Hint Resolve kinding_typ_subst_l : typ_subst.
+Hint Resolve kinding_typ_substs : typ_subst.
+Hint Resolve kinding_typ_substs_l : typ_subst.
+Hint Resolve kindings_typ_subst : typ_subst.
+
+Lemma kinding_sch_open : forall E M Ts,
+  kinding_scheme E M ->
+  kindings E (sch_arity M) Ts (sch_kinds M) ->
+  kinding E (sch_open M Ts) knd_type.
+Proof.
+  introv Hks Hkt.
+  destruct Hks as [L Hks].
+  pick_freshes (sch_arity M) Xs.
+  destruct Hks with Xs as [Hkd Hkk]; auto.
+  lets Hlx : (fresh_length _ _ _ Fr).
+  lets Hlk : (proj1 (proj32 (kindings_regular Hkt))).
+  rewrite* (@typ_substs_intro_sch M Xs Ts).
+  unfold sch_open_vars.
+  apply kinding_typ_substs_l
+    with (Js := sch_kinds M) (n := sch_arity M); auto.
+Qed.
+
+Hint Resolve kinding_sch_open : kinding.
+ 
+(* *************************************************************** *)
+(** Kinding of schemes with no parameters *)
+
+Lemma kinding_scheme_no_params : forall E T M,
+    kinding E T knd_type ->
+    M = Sch nil T ->
+    kinding_scheme E M.
+Proof.
+  introv Hk Heq.
+  subst.
+  exists_fresh Xs Hf.
+  simpl.
+  destruct (List.length_zero_iff_nil Xs) as [Hlz _].
+  rewrite (Hlz (eq_sym (fresh_length _ _ _ Hf))).
+  rewrite singles_nil.
+  rewrite map_empty.
+  rewrite concat_empty_r.
+  unfold typ_open_vars.
+  rewrite* <- (@typ_open_type T (typ_fvars nil)).
+Qed.
 
 (* *************************************************************** *)
-(** Manipulating well-kinded environments *)
+(** * Properties of well-kinded environments *)
 
 Lemma kinding_env_shorten : forall E G,
     kinding_env (E & G) ->
@@ -218,26 +356,58 @@ Proof.
     subst*.
 Qed.
 
-Hint Resolve kinding_env_shorten.
-
 Lemma kinding_env_kinds : forall E n Ks Xs,
     kinding_env E ->
     (fresh (dom E) n Xs) ->
-    length Ks = n ->
+    kinds n Ks ->
     kinding_env (E & Xs ~::* Ks).
 Proof.
   introv Hk Hf Hlk.
   lets Hlx : (eq_sym (fresh_length _ _ _ Hf)).
   gen Ks n.
+  unfold kinds.
   induction Xs; destruct Ks;
-    intros; subst; tryfalse; rew_kinds*.
+    introv Hf [Hlk Hkd] Hlx; subst; tryfalse; rew_kinds*.
   apply kinding_env_kind.
-  - eapply IHXs; intuition.
+  - apply IHXs with (length Ks); auto.
     destruct* Hf.
+    inversion Hkd.
+    split; auto.
+  - inversion Hkd.
+    auto.
   - eapply fresh_kinds; auto.
 Qed.
 
 Hint Resolve kinding_env_kinds.
+
+Lemma kinding_env_typ_push_inv : forall E x M,
+    kinding_env (E & x ~: M) ->
+    kinding_env E /\ x # E /\ kinding_scheme E M.
+Proof.
+  introv H.
+  inverts H as H1 H2 H3 H4.
+  - false (empty_push_inv H1).
+  - destruct (eq_push_inv H4) as [_ [Hv _]].
+    false Hv.
+  - destruct (eq_push_inv H4) as [Hx [Hv He]].
+    inversion Hv.
+    subst.
+    easy.
+Qed.
+
+Lemma kinding_env_kind_push_inv : forall E x K,
+    kinding_env (E & x ~:: K) ->
+    kinding_env E /\ x # E.
+Proof.
+  introv H.
+  inverts H as H1 H2 H3 H4.
+  - false (empty_push_inv H1).
+  - destruct (eq_push_inv H4) as [Hx [_ He]].
+    subst.
+    easy.
+  - destruct (eq_push_inv H4) as [_ [Hv _]].
+    false Hv.
+Qed.
 
 Lemma kinding_scheme_from_env : forall E x M,
     kinding_env E ->
@@ -247,44 +417,138 @@ Proof.
   introv He Hb.
   induction E using env_ind; rew_env_concat.
   - false (binds_empty_inv Hb).
-  - destruct (binds_push_inv Hb)
-      as [ [ Hvar Hbind ] | [ Hvar Hbind ] ].
-    + { subst.
-        inversion He.
-        - false (empty_push_inv H0).
-        - destruct (eq_push_inv H) as [_ [Heq _]].
-          false Heq.
-        - destruct (eq_push_inv H) as [_ [Heq _]].
-          inversion Heq.
-          subst.
-          apply* kinding_scheme_weakening_l. }
-    + apply* kinding_scheme_weakening_l.
+  - destruct (binds_push_inv Hb); jauto_set.
+    + subst.
+      destruct (kinding_env_typ_push_inv He).
+      jauto_set.
+      auto with weaken.
+    + eauto using kinding_env_shorten with weaken.
 Qed.
 
-Hint Resolve kinding_scheme_from_env.
+Hint Resolve kinding_scheme_from_env : kinding.
+
+Lemma kinding_env_well_scoped : forall E F X B,
+    kinding_env (E & X ~ B & F) ->
+    X \notin (env_fv E).
+Proof.
+  introv Hkef Hfv.
+  assert (kinding_env E) as Hke by eauto using kinding_env_shorten. 
+  lets Hd : (kinding_env_closed Hke Hfv).
+  assert (ok (E & X ~ B & F)) as Hok by auto.
+  apply ok_middle_inv in Hok.
+  iauto.
+Qed.
 
 (* *************************************************************** *)
-(** Kinding of schemes with no parameters *)
+(** Not affected by type bindings *)
 
-Lemma kinding_scheme_no_params : forall E T M,
-    kinding E T kind_type ->
-    M = Sch nil T ->
-    kinding_scheme E M.
+Lemma kinding_env_bind_typ : forall E F x M,
+    kinding_env (E & x ~: M & F) ->
+    kinding_env (E & F).
 Proof.
-  introv Hk Heq.
-  subst.
-  exists_fresh Xs Hf.
-  simpl.
-  destruct (List.length_zero_iff_nil Xs) as [Hlz _].
-  rewrite (Hlz (eq_sym (fresh_length _ _ _ Hf))).
-  rewrite singles_nil.
-  rewrite map_empty.
-  rewrite concat_empty_r.
-  unfold typ_open_vars.
-  rewrite* <- (@typ_open_type T (typ_fvars nil)).
+  introv Hk.
+  induction F using env_ind.
+  - rewrite concat_empty_r.
+    eauto using kinding_env_shorten.
+  - rewrite concat_assoc in *.
+    inversion Hk.
+    + apply empty_push_inv in H0.
+      tryfalse.
+    + destruct (eq_push_inv H) as [Ha [Hb Hc]].
+      subst.
+      apply kinding_env_kind; auto.
+    + destruct (eq_push_inv H) as [Ha [Hb Hc]].
+      subst; eauto using kinding_scheme_bind_typ.
 Qed.
 
-Hint Resolve kinding_env_shorten.
+Hint Resolve kinding_env_bind_typ : bind_typ.
+
+(* *************************************************************** *)
+(** Preserved by type substitution *)
+
+Lemma kinding_env_typ_subst : forall E F X K T,
+  kinding_env (E & X ~:: K & F) -> 
+  kinding E T K -> 
+  kinding_env (E & (environment_subst X T F)).
+Proof.
+  introv He Hk.
+  induction F using env_ind.
+  - rewrite environment_subst_empty.
+    rewrite concat_empty_r.
+    eauto using kinding_env_shorten.
+  - rewrite environment_subst_push.
+    rewrite concat_assoc.
+    rewrite concat_assoc in He.
+    destruct v; simpl binding_subst.
+    + { destruct (kinding_env_kind_push_inv He).
+        apply kinding_env_kind; auto.
+        - lets Hee : (kinding_env_regular He).
+          apply kind_from_env with
+            (E := E & X ~:: K & F & x ~:: k)
+            (x := x); auto.
+        - rewrite dom_concat.
+          rewrite dom_environment_subst.
+          auto. }
+    + { destruct (kinding_env_typ_push_inv He) as [H1 [H2 H3]].
+        apply kinding_env_typ; auto.
+        - apply kinding_scheme_typ_subst with K; auto.
+        - rewrite dom_concat.
+          rewrite* dom_environment_subst. }
+Qed.
+
+Hint Resolve kinding_env_typ_subst: typ_subst.
+
+(* *************************************************************** *)
+(** Uniqueness *)
+
+Lemma kinding_unique : forall E T K1 K2,
+    kinding E T K1 ->
+    kinding E T K2 ->
+    K1 = K2.
+Proof.
+  introv Hk1 Hk2.
+  gen K2.
+  induction Hk1; introv Hk2; inversion Hk2; subst; auto.
+  - lets Hke : (binds_func H0 H4).
+    inversion Hke; auto.
+  - lets Hke1 : (IHHk1_1 _ H4).
+    lets Hke2 : (IHHk1_2 _ H6).
+    inversion Hke1.
+    inversion Hke2.
+    reflexivity.
+Qed.
+
+(* *************************************************************** *)
+(** Extract kinding from [typ_or] *)
+
+Lemma kinding_or_inv_l : forall E T1 T2 cs1 cs2,
+    kinding E (typ_or T1 T2) (knd_row cs1) ->
+    kinding E T2 (knd_row cs2) ->
+    kinding E T1 (knd_row (cons_diff cs1 cs2)).
+Proof.
+  introv Hk1 Hk2.
+  inversion Hk1.
+  assert (knd_row cs2 = knd_row cs3) as Heq
+    by eauto using kinding_unique.
+  inversion Heq.
+  subst.
+  rewrite cons_diff_union; auto.
+Qed.  
+
+Lemma kinding_or_inv_r : forall E T1 T2 cs1 cs2,
+    kinding E (typ_or T1 T2) (knd_row cs1) ->
+    kinding E T1 (knd_row cs2) ->
+    kinding E T2 (knd_row (cons_diff cs1 cs2)).
+Proof.
+  introv Hk1 Hk2.
+  inversion Hk1.
+  assert (knd_row cs0 = knd_row cs2) as Heq
+    by eauto using kinding_unique.
+  inversion Heq.
+  subst.
+  rewrite cons_union_commutative.
+  rewrite cons_diff_union; auto with constrs.
+Qed.  
 
 (* *************************************************************** *)
 (** * Properties of type equality *)
@@ -300,8 +564,6 @@ Proof.
   induction* Hk.
 Qed.
 
-Hint Resolve type_equal_refl.
-
 (* *************************************************************** *)
 (** Symmetry *)
 
@@ -310,36 +572,39 @@ Lemma type_equal_symm : forall E T1 T2 K,
     type_equal E T2 T1 K.
 Proof.
   introv He.
-  induction* He.
+  induction He; eauto.
+  - assert (cons_union cs1 cs2 = cons_union cs2 cs1)
+      as comm by constrs.
+    rewrite comm.
+    auto with constrs.
 Qed.
-
-Hint Resolve type_equal_symm.
 
 (* *************************************************************** *)
 (** Idempotence of join and meet *)
 
-Lemma type_equal_join_idempotent : forall E T,
-    kinding E T kind_row ->
-    type_equal E (typ_join T T) T kind_row.
+Lemma type_equal_join_idempotent : forall E T cs,
+    kinding E T (knd_row cs) ->
+    type_equal E (typ_join T T) T (knd_row cs).
 Proof.
   introv Hk.
   apply type_equal_trans
-    with (typ_join T (typ_meet T typ_top)); auto.
+    with (typ_join T (typ_meet T (typ_top cs)));
+    auto using type_equal_refl.
 Qed.
 
-Hint Resolve type_equal_join_idempotent.
-
-Lemma type_equal_meet_idempotent : forall E T,
-    kinding E T kind_row ->
-    type_equal E (typ_meet T T) T kind_row.
+Lemma type_equal_meet_idempotent : forall E T cs,
+    kinding E T (knd_row cs) ->
+    type_equal E (typ_meet T T) T (knd_row cs).
 Proof.
   introv Ht.
   apply type_equal_trans
-    with (typ_meet T (typ_join T typ_bot)); auto.
+    with (typ_meet T (typ_join T (typ_bot cs)));
+    auto using type_equal_refl.
 Qed.
 
+Hint Resolve type_equal_join_idempotent.
 Hint Resolve type_equal_meet_idempotent.
-
+    
 (* *************************************************************** *)
 (** Well-kindedness *)
 
@@ -348,7 +613,13 @@ Lemma type_equal_kinding : forall E T1 T2 K,
     kinding E T1 K /\ kinding E T2 K.
 Proof.
   introv He.
-  induction* He.
+  induction He; split; intuition auto with constrs.
+  - rewrite cons_union_commutative.
+    auto with constrs.
+  - rewrite cons_union_associative.
+    auto with constrs.
+  - rewrite cons_union_associative.
+    auto with constrs.
 Qed.
 
 Hint Extern 1 (kinding ?E ?T ?K) =>
@@ -357,7 +628,20 @@ Hint Extern 1 (kinding ?E ?T ?K) =>
       apply (proj1 (type_equal_kinding H))
   | H: type_equal E _ T K |- _ =>
       apply (proj2 (type_equal_kinding H))
-  end.
+  end : kinding.
+
+(* *************************************************************** *)
+(** Not affected by type bindings *)
+
+Lemma type_equal_bind_typ : forall E F T1 T2 K x S,
+    type_equal (E & x ~: S & F) T1 T2 K ->
+    type_equal (E & F) T1 T2 K.
+Proof.
+  introv He.
+  gen_eq G : (E & x ~: S & F).
+  induction He; intros; subst;
+    eauto 6 using type_equal_refl with bind_typ; auto with constrs.
+Qed.  
 
 (* *************************************************************** *)
 (** Preserved by type substitution *)
@@ -370,7 +654,8 @@ Lemma type_equal_typ_subst : forall E F X T1 T2 S K J,
 Proof.
   introv Hkt Hks.
   gen_eq G: (E & X ~:: J & F).
-  inductions Hkt; introv Heq; subst; simpl typ_subst; eauto.
+  inductions Hkt; introv Heq; subst;
+    simpl typ_subst; eauto 6 using type_equal_refl with typ_subst; auto with constrs.
   - case_var.
     + apply type_equal_refl.
       lets Hb : (binds_middle_eq_inv H0 (ok_from_environment H)).
@@ -383,7 +668,7 @@ Proof.
         - auto. }
 Qed.
 
-Hint Resolve type_equal_typ_subst.
+Hint Resolve type_equal_typ_subst : typ_subst.
 
 (* *************************************************************** *)
 (** Weakening *)
@@ -394,13 +679,28 @@ Lemma type_equal_weakening : forall E F G T1 T2 K,
    type_equal (E & F & G) T1 T2 K.
 Proof.
   introv Heq Henv.
-  inductions Heq; auto.
+  inductions Heq; auto with weaken.
   - apply type_equal_trans with T2.
     + apply IHHeq1 with (E0 := E) (G0 := G); auto.
     + apply IHHeq2 with (E0 := E) (G0 := G); auto.
 Qed.
 
-Hint Resolve type_equal_weakening.
+Hint Resolve type_equal_weakening : weaken.
+
+(* *************************************************************** *)
+(** Kind can be replaced *)
+
+Lemma type_equal_replace_kind : forall E T1 T2 K1 K2,
+    kinding E T1 K1 ->
+    type_equal E T1 T2 K2 ->
+    type_equal E T1 T2 K1.
+Proof.
+  introv Hk He.
+  assert (K1 = K2) as Heq
+    by eauto using kinding_unique with kinding.
+  rewrite Heq.
+  assumption.
+Qed.    
 
 (* *************************************************************** *)
 (** * Properties of Subtyping *)
@@ -409,11 +709,11 @@ Hint Resolve type_equal_weakening.
 (** Reflexivity *)
 
 Lemma subtype_refl : forall E T,
-  kinding E T kind_row -> 
+  kinding E T (knd_row cons_universe) -> 
   subtype E T T.
 Proof.
   introv Hk.
-  inversion Hk; unfold subtype; auto.
+  inversion Hk; subst; unfold subtype; auto using type_equal_symm.
 Qed.
 
 (* *************************************************************** *)
@@ -428,9 +728,12 @@ Proof.
   unfold subtype in *.
   destruct (type_equal_kinding H23) as [ _ Hk ].
   inversion Hk; subst.
-  apply type_equal_trans with (typ_join T1 T2); auto.
-  apply type_equal_trans with (typ_join T1 (typ_join T2 T3)); auto.
-  apply type_equal_trans with (typ_join (typ_join T1 T2) T3); auto.
+  apply type_equal_trans with (typ_meet T1 T2); auto.
+  apply type_equal_trans with (typ_meet T1 (typ_meet T2 T3));
+    auto using type_equal_refl with kinding.
+  apply type_equal_trans with (typ_meet (typ_meet T1 T2) T3);
+    auto with kinding.
+  auto using type_equal_refl, type_equal_symm.
 Qed.
 
 (* *************************************************************** *)
@@ -439,12 +742,14 @@ Qed.
 Lemma subtype_antisymm : forall E T1 T2,
     subtype E T1 T2 ->
     subtype E T2 T1 ->
-    type_equal E T1 T2 kind_row.
+    type_equal E T1 T2 (knd_row cons_universe).
 Proof.
   introv H12 H21.
   unfold subtype in *.
-  apply type_equal_trans with (typ_join T1 T2); auto.
-  apply type_equal_trans with (typ_join T2 T1); auto.
+  apply type_equal_trans with (typ_meet T1 T2); auto.
+  apply type_equal_trans with (typ_meet T2 T1);
+    auto using type_equal_symm.
+  auto with kinding.
 Qed.
 
 (* *************************************************************** *)
@@ -452,7 +757,8 @@ Qed.
 
 Lemma subtype_kinding : forall E T1 T2,
     subtype E T1 T2 ->
-    kinding E T1 kind_row /\ kinding E T2 kind_row.
+    kinding E T1 (knd_row cons_universe)
+    /\ kinding E T2 (knd_row cons_universe).
 Proof.
   introv He.
   destruct (type_equal_kinding He) as [ Hk Hj ].
@@ -460,13 +766,13 @@ Proof.
   inversion* Hj.
 Qed.
 
-Hint Extern 1 (kinding ?E ?T kind_row) =>
+Hint Extern 1 (kinding ?E ?T (knd_row cons_universe)) =>
   match goal with
   | H: subtype E T _ |- _ =>
       apply (proj1 (subtype_kinding H))
   | H: subtype E _ T |- _ =>
       apply (proj2 (subtype_kinding H))
-  end.
+  end : kinding.
 
 (* *************************************************************** *)
 (** Weakening *)
@@ -480,7 +786,22 @@ Proof.
   apply* type_equal_weakening.
 Qed.
 
-Hint Resolve subtype_weakening.
+Hint Resolve subtype_weakening : weaken.
+
+(* *************************************************************** *)
+(** Not affected by type bindings *)
+
+Lemma subtype_bind_typ : forall E F T1 T2 x S,
+    subtype (E & x ~: S & F) T1 T2 ->
+    subtype (E & F) T1 T2.
+Proof.
+  unfold subtype.
+  introv He.
+  eapply type_equal_bind_typ.
+  apply He.
+Qed.  
+
+Hint Resolve subtype_bind_typ : bind_typ.
 
 (* *************************************************************** *)
 (** Preserved by type substitution *)
@@ -498,10 +819,421 @@ Proof.
   auto.
 Qed.
 
-Hint Resolve subtype_typ_subst.
+Hint Resolve subtype_typ_subst : typ_subst.
+
+(* *************************************************************** *)
+(** TODO: Describe and rename these lemmas *)
+
+Inductive row_projection : env -> typ -> knd -> constructors -> typ -> Prop :=
+  | row_projection_identity : forall E cs T,
+      kinding E T (knd_row cs) ->
+      row_projection E T (knd_row cs) cs T
+  | row_projection_or_l : forall E cs1 cs2 cs3 T1 T2 T1',
+      cons_subset cs1 cs2 ->
+      cons_disjoint cs2 cs3 ->
+      row_projection E T1 (knd_row cs2) cs1 T1' ->
+      kinding E T2 (knd_row cs3) ->
+      row_projection E (typ_or T1 T2) (knd_row (cons_union cs2 cs3)) cs1 T1'
+  | row_projection_or_r : forall E cs1 cs2 cs3 T1 T2 T2',
+      cons_subset cs1 cs3 ->
+      cons_disjoint cs2 cs3 ->
+      kinding E T1 (knd_row cs2) ->
+      row_projection E T2 (knd_row cs3) cs1 T2' ->
+      row_projection E (typ_or T1 T2) (knd_row (cons_union cs2 cs3)) cs1 T2'
+  | row_projection_or_both : forall E cs1 cs2 cs3 T1 T1' T2 T2',
+      cons_subset cs1 (cons_union cs2 cs3) ->
+      cons_non_empty (cons_inter cs1 cs2) ->
+      cons_non_empty (cons_inter cs1 cs3) ->
+      cons_disjoint cs2 cs3 ->
+      row_projection E T1 (knd_row cs2) (cons_inter cs1 cs2) T1' ->
+      row_projection E T2 (knd_row cs3) (cons_inter cs1 cs3) T2' ->
+      row_projection E (typ_or T1 T2) (knd_row (cons_union cs2 cs3)) cs1 (typ_or T1' T2')
+  | row_projection_meet : forall E K cs T1 T2 T3 T4,
+      row_projection E T1 K cs T3 ->
+      row_projection E T2 K cs T4 ->
+      row_projection E (typ_meet T1 T2) K cs (typ_meet T3 T4)
+  | row_projection_join : forall E K cs T1 T2 T3 T4,
+      row_projection E T1 K cs T3 ->
+      row_projection E T2 K cs T4 ->
+      row_projection E (typ_join T1 T2) K cs (typ_join T3 T4)
+  | row_projection_bot : forall E cs1 cs2,
+      environment E ->
+      cons_non_empty cs1 ->
+      cons_subset cs1 cs2 ->
+      row_projection E (typ_bot cs2) (knd_row cs2) cs1 (typ_bot cs1)
+  | row_projection_top : forall E cs1 cs2,
+      environment E ->
+      cons_non_empty cs1 ->
+      cons_subset cs1 cs2 ->
+      row_projection E (typ_top cs2) (knd_row cs2) cs1 (typ_top cs1).
+
+Hint Constructors row_projection.
+
+Lemma row_projection_kinding_ind : forall E cs T K T',
+    row_projection E T K cs T' ->
+    (exists cs', K = knd_row cs') /\ kinding E T K /\ kinding E T' (knd_row cs).
+Proof.
+  introv Hr.
+  induction Hr; splits; iauto.
+  - replace cs1
+        with (cons_union (cons_inter cs1 cs2)
+                         (cons_inter cs1 cs3))
+    by constrs.
+    auto with constrs.
+  - destruct IHHr1 as [[cs' Heq] ?].
+    rewrite Heq in *.
+    iauto.
+  - destruct IHHr1 as [[cs' Heq] ?].
+    rewrite Heq in *.
+    iauto.
+  - auto with constrs.
+  - auto with constrs.
+Qed.
+
+Lemma row_projection_kinding : forall E cs T K T',
+    row_projection E T K cs T' ->
+    kinding E T K /\ kinding E T' (knd_row cs).
+Proof.
+  introv Hpr.
+  apply row_projection_kinding_ind in Hpr.
+  iauto.
+Qed.
+
+Hint Extern 1 (kinding ?E ?T (knd_row ?cs)) =>
+  match goal with
+  | H: row_projection E T (knd_row ?cs) _ _ |- _ =>
+      apply (proj1 (row_projection_kinding H))
+  | H: row_projection E _ _ cs T |- _ =>
+      apply (proj2 (row_projection_kinding H))
+  end : kinding.
+
+Lemma row_projection_idem : forall E cs T T',
+    row_projection E T (knd_row cs) cs T' ->
+    T = T'.
+Proof.
+  introv Hpr.
+  gen_eq K : (knd_row cs).
+  induction Hpr; intro; auto.
+  - assert (cons_non_empty cs3) by auto.
+    apply row_projection_kinding in Hpr.
+    assert (cons_non_empty cs2) by iauto.
+    inversion H2; subst.
+    false.
+    constrs.
+  - assert (cons_non_empty cs2) by auto.
+    apply row_projection_kinding in Hpr.
+    assert (cons_non_empty cs3) by iauto.
+    inversion H2; subst.
+    false.
+    constrs.
+  - inversion H3; subst.
+    replace T1' with T1 by auto with constrs.
+    replace T2' with T2 by auto with constrs.
+    auto.
+  - replace T3 with T1 by auto.
+    replace T4 with T2 by auto.
+    auto.
+  - replace T3 with T1 by auto.
+    replace T4 with T2 by auto.
+    auto.
+  - inversion H2.
+    auto.
+  - inversion H2.
+    auto.
+Qed.
+
+Ltac equal_kinds :=
+  repeat
+    match goal with
+    | [ Hr : row_projection ?E ?T (knd_row ?cs) _ _ |- _ ] =>
+      match goal with
+      | [ Hk : kinding E T (knd_row cs) |- _ ] =>
+        fail 1
+      | _ =>
+        let Hk := fresh "Hk" in
+        assert (kinding E T (knd_row cs)) as Hk
+            by (apply (proj1 (row_projection_kinding Hr)))
+      end
+    | [ He : type_equal ?E ?T _ (knd_row ?cs) |- _ ] =>
+      match goal with
+      | [ Hk : kinding E T (knd_row cs) |- _ ] =>
+        fail 1
+      | _ =>
+        let Hk := fresh "Hk" in
+        assert (kinding E T (knd_row cs)) as Hk
+            by (apply (proj1 (type_equal_kinding He)))
+      end
+    | [ He : type_equal ?E _ ?T (knd_row ?cs) |- _ ] =>
+      match goal with
+      | [ Hk : kinding E T (knd_row cs) |- _ ] =>
+        fail 1
+      | _ =>
+        let Hk := fresh "Hk" in
+        assert (kinding E T (knd_row cs)) as Hk
+            by (apply (proj2 (type_equal_kinding He)))
+      end
+    end;
+  repeat
+    match goal with
+    | [ Hk1 : kinding ?E ?T (knd_row ?cs1),
+        Hk2 : kinding ?E ?T (knd_row ?cs2) |- _ ] =>
+      match goal with
+      | [ Heq : (knd_row cs1) = (knd_row cs2) |- _ ] =>
+        fail 1
+      | [ Heq : (knd_row cs2) = (knd_row cs1) |- _ ] =>
+        fail 1
+      | _ =>
+        let Heq := fresh "Heq" in
+        assert ((knd_row cs1) = (knd_row cs2)) as Heq
+            by apply (kinding_unique Hk1 Hk2);
+        inversion Heq
+      end
+    end;
+  subst.
+
+Lemma row_projection_unique : forall E cs T K T' T'',
+    row_projection E T K cs T' ->
+    row_projection E T K cs T'' ->
+    T' = T''.
+Proof.
+  introv Hpr1 Hpr2.
+  gen T''.
+  induction Hpr1; introv Hpr2.
+  - eauto using row_projection_idem.
+  - inversion Hpr2; subst; equal_kinds; auto.
+    + assert (cons_non_empty cs3) by auto.
+      false.
+      constrs.
+    + assert (cons_non_empty cs1).
+      { apply row_projection_kinding in Hpr1.
+        iauto. }
+      false.
+      constrs.
+    + false.
+      constrs.
+  - inversion Hpr2; subst; equal_kinds; auto.
+    + assert (cons_non_empty cs2) by auto.
+      false.
+      constrs.
+    + assert (cons_non_empty cs1).
+      { apply row_projection_kinding in Hpr1.
+        iauto. }
+      false.
+      constrs.
+    + false.
+      constrs.
+  - inversion Hpr2; subst.
+    + replace (cons_inter (cons_union cs2 cs3) cs2)
+        with cs2 in Hpr1_1 by constrs.
+      replace (cons_inter (cons_union cs2 cs3) cs3)
+        with cs3 in Hpr1_2 by constrs.
+      apply row_projection_idem in Hpr1_1.
+      apply row_projection_idem in Hpr1_2.
+      subst.
+      reflexivity.
+    + equal_kinds.
+      false.
+      constrs.
+    + equal_kinds.
+      false.
+      constrs.
+    + equal_kinds.
+      f_equal; auto.
+  - inversion Hpr2; subst.
+    + apply row_projection_idem in Hpr1_1.
+      apply row_projection_idem in Hpr1_2.
+      subst.
+      reflexivity.
+    + f_equal; auto.
+  - inversion Hpr2; subst.
+    + apply row_projection_idem in Hpr1_1.
+      apply row_projection_idem in Hpr1_2.
+      subst.
+      reflexivity.
+    + f_equal; auto.
+  - inversion Hpr2; subst; auto.
+  - inversion Hpr2; subst; auto.
+Qed.
+
+Lemma type_equal_project : forall E cs1 T1 T2 T1' K,
+    type_equal E T1 T2 K ->
+    row_projection E T1 K cs1 T1' ->
+    exists T2',
+    row_projection E T2 K cs1 T2' /\
+    type_equal E T1' T2' (knd_row cs1).
+Proof.
+  introv He Hpr.
+  gen T1'.
+  induction He; introv Hpr.
+  - eauto using type_equal_refl with kinding.
+  - inversion Hpr; subst.
+    exists (typ_constructor c T').
+    auto with kinding.
+  - inversion Hpr; subst.
+    + exists (typ_or T1' T2').
+      auto with kinding.
+    + equal_kinds.
+      destruct (IHHe1 _ H6).
+      
+
+Lemma subtype_or_project : forall E cs1 cs2 T1 T1' T2 T2',
+    cons_disjoint cs1 cs2 ->
+    kinding E T1 (knd_row cs1) ->
+    kinding E T2 (knd_row cs2) ->
+    kinding E T1' (knd_row cs1) ->
+    kinding E T2' (knd_row cs2) ->
+    type_equal E (typ_or T1 T2) (typ_or T1' T2')
+               (knd_row (cons_union cs1 cs2)) ->
+    type_equal E T1 T1' (knd_row cs1)
+    /\ type_equal E T2 T2' (knd_row cs2).
+Proof.
+  introv Hd Hk1 Hk2 Hk3 Hk4 He.
+  remember (typ_or T1 T2) as Tor1.
+  remember (typ_or T1' T2') as Tor2.
+  remember (knd_row cs1) as K1.
+  remember (knd_row cs2) as K2.
+  remember (knd_row (cons_union cs1 cs2)) as Ku.
+  induction He; subst; tryfalse.
+  - inversion HeqTor1.
+    inversion HeqTor2.
+    subst.
+    intuition eauto using type_equal_replace_kind.
+  - 
+  - inversion HeqTor1.
+    inversion HeqTor2.
+    rewrite <- H3 in *.
+    rewrite <- H6 in *.
+    assert (knd_row cs1 = knd_row cs2)
+      as Heq by eauto using kinding_unique.
+    inversion Heq.
+    subst.
+    skip.
+  - inversion HeqTor1.
+    inversion HeqTor2.
+    subst.
+    inversion Hk2; tryfalse.
+    subst.
+    assert (knd_row cs6 = knd_row (cons_union cs5 cs6))
+      as Heq by eauto using kinding_unique.
+    skip.
+  - inversion HeqTor1.
+    inversion HeqTor2.
+    subst.
+    inversion Hk4; tryfalse.
+    subst.
+    assert (knd_row cs6 = knd_row (cons_union cs5 cs6))
+      as Heq by eauto using kinding_unique.
+    skip.
+Foo.
+    
+Lemma subtype_or_split_l : forall E c cs T1 T2 T3,
+    kinding E T1 (knd_row (cons_finite cs)) ->
+    kinding E T2 (knd_row (cons_cofinite cs)) ->
+    kinding E T3 knd_type ->
+    mem c cs ->
+    subtype E (typ_or (typ_constructor c T3)
+                      (typ_bot (cons_cofinite \{c})))
+            (typ_or T1 T2) ->
+    subtype E (typ_or (typ_constructor c T3)
+                      (typ_bot (cons_cofinite \{c})))
+            (typ_or T1 (typ_bot (cons_cofinite cs))).
+Proof.
+  unfold subtype.
+  introv Hk1 Hk2 Hk3 Hin Hs.
+  assert (type_equal E
+            (typ_or (typ_constructor c T3)
+                    (typ_bot (cons_cofinite \{c})))
+            (typ_or (typ_or
+                       (typ_constructor c T3)
+                       (typ_bot (cons_finite (cs \- \{c}))))
+                    (typ_bot (cons_cofinite cs)))
+            (knd_row cons_universe)).
+  { apply type_equal_trans with
+      (typ_or (typ_constructor c T3)
+              (typ_or (typ_bot (cons_finite (cs \- \{c})))
+                      (typ_bot (cons_cofinite cs)))).
+    - rewrite <- cons_union_universe with \{c}.
+      apply type_equal_or; auto using type_equal_refl with constrs.
+      replace (cons_cofinite \{c})
+        with (cons_union (cons_finite (cs \- \{c}))
+                         (cons_cofinite cs))
+        by constrs.
+      apply type_equal_or_bot_r; auto with constrs.
+    - replace cons_universe
+        with (cons_union (cons_finite \{c})
+                (cons_union (cons_finite (cs \- \{c}))
+                            (cons_cofinite cs)))
+        by constrs.
+      apply type_equal_or_associative_l; auto with constrs. }
+  rewrite <- cons_union_universe with cs in *.
+  apply type_equal_trans with
+    (typ_or (typ_or (typ_constructor c T3)
+                    (typ_bot (cons_finite (cs \- \{c}))))
+            (typ_bot (cons_cofinite cs))); auto.
+  apply type_equal_trans with
+    (typ_meet
+       (typ_or (typ_or (typ_constructor c T3)
+                    (typ_bot (cons_finite (cs \- \{c}))))
+            (typ_bot (cons_cofinite cs)))
+       (typ_or T1 (typ_bot (cons_cofinite cs))));
+    auto using type_equal_symm, type_equal_refl with constrs.
+  apply type_equal_trans with
+    (typ_or
+       (typ_meet (typ_or (typ_constructor c T3)
+                    (typ_bot (cons_finite (cs \- \{c}))))
+                 T1)
+       (typ_meet (typ_bot (cons_cofinite cs))
+                 (typ_bot (cons_cofinite cs)))); auto.
+  - apply type_equal_or; auto with constrs.
+    +         
+    + eauto using type_equal_symm, type_equal_meet_idempotent.
+  - apply type_equal_or_meet_distribution_l; auto with constrs.
+    replace (cons_finite cs)
+        with (cons_union (cons_finite \{c})
+                (cons_finite (cs \- \{c})))
+        by auto with constrs.
+    apply kinding_or; auto with constrs. 
+Qed.
+
+Lemma subtype_or_split_r : forall E cs T1 T2,
+    kinding E T1 (knd_row (cons_finite cs)) ->
+    kinding E T2 (knd_row (cons_cofinite cs)) ->
+    subtype E (typ_or T1 T2) (typ_or (typ_bot (cons_finite cs)) T2).
+Proof.
+  unfold subtype.
+  introv Hk1 Hk2.
+  rewrite <- cons_union_universe with cs.
+  apply type_equal_trans with
+    (typ_or (typ_meet T1 (typ_bot (cons_finite cs)))
+            (typ_meet T2 T2)).
+  - apply type_equal_or;
+      auto using type_equal_meet_idempotent, type_equal_symm
+        with constrs.
+  - apply type_equal_or_meet_distribution_l; auto with constrs.
+Qed.
 
 (* *************************************************************** *)
 (** * Properties of typing *)
+
+Lemma typing_scheme_no_params : forall E e T,
+    typing E e T ->
+    typing_scheme E e (Sch nil T).
+Proof.
+  introv Ht.
+  unfold typing_scheme, sch_arity.
+  simpl.
+  exists_fresh Xs Hfr.
+  apply fresh_length in Hfr.
+  apply eq_sym in Hfr.
+  rewrite List.length_zero_iff_nil in Hfr.
+  subst.
+  rewrite singles_nil.
+  rewrite map_empty.
+  rewrite concat_empty_r.
+  unfold sch_open_vars, typ_open_vars.
+  simpl.
+  rewrite* <- typ_open_type.
+Qed.
 
 Lemma typing_kinding_env : forall E e T,
     typing E e T ->
@@ -510,43 +1242,32 @@ Proof.
   introv Ht.
   induction* Ht.
   - pick_fresh x.
-    eapply kinding_env_shorten in H1; auto.
+    eapply kinding_env_shorten in H0; auto.
   - pick_freshes (sch_arity M) Xs.
     eapply kinding_env_shorten in H0; auto.
 Qed.
 
-Hint Resolve typing_kinding_env.
+Hint Resolve typing_kinding_env : kinding.
 
 Lemma typing_kinding : forall E e T,
     typing E e T ->
-    kinding E T kind_type.
+    kinding E T knd_type.
 Proof.
   introv Ht.
-  induction* Ht.
-  - assert (kinding_scheme E M).
-    { apply kinding_scheme_from_env with x; auto. }
-    destruct H2 as [L Hs].
-    unfold sch_open.
-    pick_freshes (sch_arity M) Xs.
-    unfold sch_fv in Fr.
-    lets Hlx : (fresh_length _ _ _ Fr).
-    lets Hlk : (proj1 (proj2 (kindings_regular H1))).
-    apply kinding_typ_substs_l
-      with (Xs := Xs) (n := sch_arity M) (Ss := Us)
-      in Hs; auto.
-    rewrite (@typ_substs_intro Xs Us _); auto.
-    rewrite* <- Hlx.
+  induction Ht; eauto with kinding.
   - apply* kinding_arrow.
     pick_fresh x.
-    eapply kinding_bind_typ in H1; auto.
+    eapply kinding_bind_typ_l in H0; auto.
   - inversion* IHHt1.
   - pick_fresh x.
-    eapply kinding_bind_typ in H2; auto.
+    eapply kinding_bind_typ_l in H2; auto.
   - pick_fresh x.
-    eapply kinding_bind_typ in H0; auto.
+    eapply kinding_bind_typ_l in H0; auto.
+  - pick_fresh x.
+    eapply kinding_bind_typ_l in H0; auto.
 Qed.
 
-Hint Resolve typing_kinding.
+Hint Resolve typing_kinding : kinding.
 
 Lemma typing_scheme_kinding : forall E e M,
     typing_scheme E e M ->
@@ -557,10 +1278,20 @@ Proof.
   eapply typing_kinding in Ht; eauto.
 Qed.  
 
-Hint Resolve typing_scheme_kinding.
+Hint Resolve typing_scheme_kinding : kinding.
 
 (* *************************************************************** *)
 (** Weakening *)
+
+Lemma fresh_dom_concat : forall (E : env) F n Xs,
+    fresh (dom E \u dom F) n Xs ->
+    fresh (dom (E & F)) n Xs.
+Proof.
+  intros.
+  rewrite* dom_concat.
+Qed.
+
+Hint Resolve fresh_dom_concat : weaken.
 
 Lemma typing_weakening : forall E F G e T,
    typing (E & G) e T -> 
@@ -570,46 +1301,351 @@ Proof.
   introv Ht.
   gen_eq EG : (E & G).
   gen E F G.
-  induction Ht; intros; subst; eauto.
-  - apply_fresh* typing_abs as y.
-    apply_ih_bind H1; auto.
-    eapply kinding_scheme_no_params in H; auto.
-    apply* kinding_env_typ.
+  induction Ht; intros; subst; eauto with weaken.
+  - apply_fresh typing_abs as y; auto with weaken.
+    apply_ih_bind H0;
+      eauto using kinding_scheme_no_params with weaken.
   - apply_fresh (@typing_let M) as Ys.
-    + apply_ih_bind H0; auto.
-      apply kinding_env_kinds with (sch_arity M); auto.
-      rewrite! dom_concat.
-      auto.
+    + apply_ih_bind H0; eauto with weaken.
     + apply_ih_bind H2; auto.
-      apply* kinding_env_typ.
+      apply kinding_env_typ; auto.
       eapply typing_scheme_kinding.
       exists_fresh Xs Hf.
-      apply_ih_bind H0; auto.
-      apply kinding_env_kinds with (sch_arity M); auto.
-      rewrite! dom_concat.
-      auto.
-  - apply_fresh* (@typing_match c) as Ys.
-    + { apply_ih_bind H0; auto.
-        apply* kinding_env_typ.
-        apply kinding_scheme_no_params with T3; auto.
-        assert (kinding (E0 & F & G)
-                  (typ_join (typ_constructor c T3) T6) kind_row)
-          by eauto.
-        inversion H6.
-        inversion H11.
-        auto. }
+      apply_ih_bind H0; eauto with weaken.
+  - let G := gather_vars in
+    eapply typing_match with (L := G) (T10 := T10);
+      eauto with weaken; introv Hf.
+    + apply_ih_bind H0; auto.
+      apply kinding_env_typ; auto.
+      apply kinding_scheme_no_params with (typ_variant T3 T4);
+        auto with weaken kinding.
     + apply_ih_bind H2; auto.
-      apply* kinding_env_typ.
-      apply kinding_scheme_no_params with (typ_variant T5 T6); auto.
-  - eapply typing_absurd; auto.
+      apply kinding_env_typ; auto.
+      apply kinding_scheme_no_params with (typ_variant T6 T7);
+        auto with weaken kinding.
+  - let G := gather_vars in
+    eapply typing_destruct with (L := G) (T3 := T3);
+      eauto with weaken; introv Hf.
+    apply_ih_bind H0; auto.
+    apply kinding_env_typ; auto.
+    apply kinding_scheme_no_params with T3; auto with weaken.
+  - eapply typing_absurd; auto with weaken.
 Qed.
-   
+
+Lemma typing_scheme_weakening : forall E F G e M,
+   typing_scheme (E & G) e M -> 
+   kinding_env (E & F & G) ->
+   typing_scheme (E & F & G) e M.
+Proof.
+  unfold typing_scheme.
+  introv [L Hs] Hk.
+  exists (L \u dom (E & F & G)).
+  introv Hf.
+  rewrite <- concat_assoc.
+  apply typing_weakening.
+  - rewrite concat_assoc.
+    apply* Hs.
+  - rewrite concat_assoc.
+    apply kinding_env_kinds with (sch_arity M); auto.
+Qed.
+
+Lemma typing_scheme_weakening_l : forall E F e M,
+   typing_scheme E e M -> 
+   kinding_env (E & F) ->
+   typing_scheme (E & F) e M.
+Proof.
+  introv Hs Hk.
+  rewrite <- concat_empty_r with (E := E) in Hs.
+  rewrite <- concat_empty_r in Hk.
+  rewrite <- concat_empty_r with (E := F).
+  rewrite concat_assoc.
+  apply* typing_scheme_weakening.
+Qed.
+
+Hint Resolve typing_weakening : weaken.
+Hint Resolve typing_scheme_weakening : weaken.
+Hint Resolve typing_scheme_weakening_l : weaken.
+
 (* *************************************************************** *)
 (** Preserved by type substitution *)
 
-Lemma typing_typ_subst : forall F Z U E t T,
-  Z \notin (env_fv E) -> 
-  type U -> 
-  E & F |= t ~: T -> 
-  E & (map (sch_subst Z U) F) |= t ~: (typ_subst Z U T).
+Lemma typing_typ_subst : forall E F X K U t T,
+  E & X ~:: K & F |= t -: T ->
+  kinding E U K ->
+  E & (environment_subst X U F) |= t -: (typ_subst X U T).
+Proof.
+  introv Ht Hk.
+  gen_eq G : (E & X ~:: K & F).
+  gen E F.
+  induction Ht; intros; subst; simpl; eauto.
+  - rewrite* sch_subst_open.
+    apply typing_var;
+      eauto using kinding_env_well_scoped with typ_subst.
+  - apply_fresh typing_abs as Y; eauto with typ_subst.
+    rewrite <- sch_subst_no_params.
+    remember (Sch nil T1) as M.
+    fold (binding_subst X U (bind_typ M)).
+    rewrite <- concat_assoc.
+    rewrite <- environment_subst_push.
+    apply H0; auto.
+    rewrite* concat_assoc.
+  - apply_fresh (@typing_let (sch_subst X U M)) as Y.
+    + rewrite <- concat_assoc.
+      rewrite <- environment_subst_kinds; auto.
+      rewrite <- sch_subst_open_vars; eauto.
+      apply H0; eauto.
+      rewrite concat_assoc.
+      auto.
+    + rewrite <- concat_assoc.
+      fold (binding_subst X U (bind_typ M)).
+      rewrite <- environment_subst_push; auto.
+      apply H2; auto.
+      rewrite concat_assoc.
+      auto.
+  - apply typing_constructor with (typ_subst X U T1);
+      eauto with typ_subst.
+    rewrite <- typ_subst_constructor.
+    rewrite <- typ_subst_bot with (X := X) (U := U).
+    rewrite <- typ_subst_or.
+    apply subtype_typ_subst with K; auto.
+  - let G := gather_vars in
+    apply typing_match with (L := G)
+      (T1 := typ_subst X U T1)
+      (T2 := typ_subst X U T2)
+      (T3 := typ_subst X U T3)
+      (T4 := typ_subst X U T4)
+      (T5 := typ_subst X U T5)
+      (T6 := typ_subst X U T6)
+      (T7 := typ_subst X U T7)
+      (T8 := typ_subst X U T8)
+      (T9 := typ_subst X U T9)
+      (T10 := typ_subst X U T10);
+      try rewrite <- typ_subst_bot with (X := X) (U := U);
+      try rewrite <- typ_subst_or;
+      eauto with typ_subst.
+    + introv Hf.
+      rewrite <- typ_subst_variant.
+      rewrite <- sch_subst_no_params.
+      remember (Sch nil (typ_variant T3 T4)) as M.
+      fold (binding_subst X U (bind_typ M)).
+      rewrite <- concat_assoc.
+      rewrite <- environment_subst_push.
+      apply H0; auto.
+      rewrite* concat_assoc.
+    + introv Hf.
+      rewrite <- typ_subst_variant.
+      rewrite <- sch_subst_no_params.
+      remember (Sch nil (typ_variant T6 T7)) as M.
+      fold (binding_subst X U (bind_typ M)).
+      rewrite <- concat_assoc.
+      rewrite <- environment_subst_push.
+      apply H2; auto.
+      rewrite* concat_assoc.
+    + rewrite <- typ_subst_row.
+      apply subtype_typ_subst with K; auto.
+  - let G := gather_vars in
+    apply typing_destruct with (L := G)
+      (T1 := typ_subst X U T1)
+      (T2 := typ_subst X U T2)
+      (T3 := typ_subst X U T3);
+      try rewrite <- typ_subst_bot with (X := X) (U := U);
+      try rewrite <- typ_subst_row;
+      eauto with typ_subst.
+    introv Hf.
+    rewrite <- sch_subst_no_params.
+    remember (Sch nil T3) as M.
+    fold (binding_subst X U (bind_typ M)).
+    rewrite <- concat_assoc.
+    rewrite <- environment_subst_push.
+    apply H0; auto.
+    rewrite concat_assoc.
+    easy.
+  - apply typing_absurd with
+      (T1 := typ_subst X U T1)
+      (T2 := typ_subst X U T2); eauto with typ_subst.
+    rewrite <- typ_subst_bot with (X := X) (U := U).
+    apply subtype_typ_subst with K; auto.
+Qed.
 
+Lemma typing_typ_substs : forall E F Xs Ks Us t T,
+  E & Xs ~::* Ks & F |= t -: T ->
+  kindings E (length Xs) Us Ks ->
+  E & (environment_substs Xs Us F) |= t -: (typ_substs Xs Us T).
+Proof.
+  introv Ht Hk.
+  destruct (kindings_length Hk) as [Hlu Hlk].
+  gen Ks Us T F.
+  induction Xs; introv Hlk Hk Hlu Ht;
+    destruct Ks; destruct Us; simpl; tryfalse.
+  - rewrite singles_nil in Ht.
+    rewrite map_empty in Ht.
+    rewrite concat_empty_r in Ht.
+    auto.
+  - inversion Hk; subst; tryfalse.
+    apply IHXs with Ks; auto.
+    apply typing_typ_subst with k.
+    + rewrite <- concat_assoc with (F := Xs ~::* Ks).
+      rewrite <- map_push.
+      rewrite <- singles_cons.
+      auto.
+    + apply kinding_weakening_l; auto.
+      assert (kinding_env (E & (a :: Xs) ~::* (k :: Ks) & F))
+        as Hke by eauto with kinding.
+      rewrite singles_cons in Hke.
+      rewrite map_push in Hke.
+      rewrite concat_assoc in Hke.
+      apply kinding_env_shorten in Hke.
+      apply kinding_env_shorten in Hke.
+      auto.
+Qed.
+
+(* *************************************************************** *)
+(** Preserved by term substitution *)
+
+Lemma typing_trm_subst : forall E F x M s t T,
+  E & x ~: M & F |= t -: T ->
+  typing_scheme E s M ->
+  E & F |= (trm_subst x s t) -: T.
+Proof.
+  introv Ht Hs.
+  gen_eq G : (E & x ~: M & F).
+  gen E F.
+  induction Ht; intros; subst; simpl; eauto with bind_typ.
+  - case_var.
+    + destruct (kindings_length H1) as [Hlu _].
+      apply binds_middle_eq_inv in H0; auto.
+      inversion H0.
+      subst.
+      destruct Hs as [L Hm].
+      pick_freshes (sch_arity M) Xs.
+      lets Hlx : (fresh_length _ _ _ Fr).
+      rewrite typ_substs_intro_sch with (Xs := Xs); iauto.
+      rewrite <- concat_empty_r with (E := E0 & F).
+      rewrite Hlx in Hlu.
+      rewrite <- environment_substs_empty
+        with (Xs := Xs) (Ts := Us); auto.
+      apply kindings_bind_typ in H1.
+      rewrite Hlx in H1.
+      apply typing_typ_substs with (sch_kinds M); auto.
+      rewrite concat_empty_r.
+      eauto 6 with weaken bind_typ.
+    + apply typing_var; eauto with bind_typ.
+      apply binds_subst with (x2 := x) (v2 := bind_typ M); auto.
+  - apply_fresh typing_abs as Y; eauto with bind_typ.
+    rewrite* trm_subst_open_var.
+    apply_ih_bind* H0.
+  - apply_fresh (@typing_let M0) as Y.
+    + apply_ih_bind* H0.
+    + rewrite* trm_subst_open_var.
+      apply_ih_bind* H2.
+  - let G := gather_vars in
+    apply typing_match with (L := G)
+      (T1 := T1) (T2 := T2) (T3 := T3) (T4 := T4)
+      (T5 := T5) (T6 := T6) (T7 := T7) (T8 := T8)
+      (T9 := T9) (T10 := T10); eauto with bind_typ.
+    + introv Hf.
+      rewrite* trm_subst_open_var.
+      apply_ih_bind* H0.
+    + introv Hf.
+      rewrite* trm_subst_open_var.
+      apply_ih_bind* H2.
+  - let G := gather_vars in
+    apply typing_destruct with (L := G)
+      (T1 := T1) (T2 := T2) (T3 := T3);
+      eauto with bind_typ.
+    introv Hf.
+    rewrite trm_subst_open_var; auto.
+    apply_ih_bind* H0.
+  - apply typing_absurd with (T1 := T1) (T2 := T2);
+      eauto with bind_typ.
+Qed.
+
+Lemma typing_trm_subst_l : forall E x M s t T,
+  E & x ~: M |= t -: T ->
+  typing_scheme E s M ->
+  E |= (trm_subst x s t) -: T.
+Proof.
+  introv Ht Hs.
+  rewrite <- concat_empty_r with (E := E & x ~: M) in Ht.
+  rewrite <- concat_empty_r with (E := E).
+  apply typing_trm_subst with M; auto.
+Qed.  
+
+(* *************************************************************** *)
+(** * Soundness *)
+
+(* *************************************************************** *)
+(** Preservation by term substitution *)
+
+Lemma preservation : preservation.
+Proof.
+  unfold preservation.
+  introv Ht Hr.
+  gen E T.
+  induction Hr; introv Ht; inversion Ht; subst; eauto.
+  - pick_fresh x.
+    rewrite trm_subst_intro with (x := x); auto.
+    apply typing_trm_subst_l with M; auto.
+    unfold typing_scheme. 
+    eauto.
+  - inversion H4.
+    subst.
+    pick_fresh x.
+    rewrite trm_subst_intro with (x := x); auto.
+    apply typing_trm_subst_l with (Sch nil S); auto.
+    auto using typing_scheme_no_params.
+  - inversion H7.
+    subst.
+    pick_fresh x.
+    rewrite trm_subst_intro with (x := x); auto.
+    apply typing_trm_subst_l with (Sch nil (typ_variant T3 T4)); auto.
+    apply typing_scheme_no_params.
+    apply typing_constructor with T0; auto.
+    apply subtype_trans with T2; auto.
+    apply subtype_trans with T1; auto.
+    apply subtype_trans with (typ_or T8 T9); auto.
+    apply subtype_trans with
+      (typ_or T8 (typ_bot (cons_cofinite (from_list cs)))); auto.
+    apply subtype_or_project_l.
+    + assert (kinding E
+             (typ_or T8 (typ_bot (cons_cofinite (from_list cs))))
+             (knd_row cons_universe)) as Hk
+        by auto with kinding.
+      rewrite <- cons_diff_universe_cofinite.
+      apply kinding_or_inv_l with
+        (typ_bot (cons_cofinite (from_list cs))); auto.
+    + assert (kinding E
+             (typ_or (typ_bot (cons_finite (from_list cs))) T9)
+             (knd_row cons_universe)) as Hk
+        by auto with kinding.
+      rewrite <- cons_diff_universe_finite.
+      apply kinding_or_inv_r with
+        (typ_bot (cons_finite (from_list cs))); auto.
+  - inversion H7.
+    subst.
+    pick_fresh x.
+    rewrite trm_subst_intro with (x := x); auto.
+    apply typing_trm_subst_l with (Sch nil (typ_variant T6 T7)); auto.
+    apply typing_scheme_no_params.
+    apply typing_constructor with T0; auto.
+    apply subtype_trans with T2; auto.
+    apply subtype_trans with T1; auto.
+    apply subtype_trans with (typ_or T8 T9); auto.
+    apply subtype_trans with
+      (typ_or (typ_bot (cons_finite (from_list cs))) T9); auto.
+    apply subtype_or_project_r.
+    + assert (kinding E
+             (typ_or T8 (typ_bot (cons_cofinite (from_list cs))))
+             (knd_row cons_universe)) as Hk
+        by auto with kinding.
+      rewrite <- cons_diff_universe_cofinite.
+      apply kinding_or_inv_l with
+        (typ_bot (cons_cofinite (from_list cs))); auto.
+    + assert (kinding E
+             (typ_or (typ_bot (cons_finite (from_list cs))) T9)
+             (knd_row cons_universe)) as Hk
+        by auto with kinding.
+      rewrite <- cons_diff_universe_finite.
+      apply kinding_or_inv_r with
+        (typ_bot (cons_finite (from_list cs))); auto.
+  - 
